src/parse/Parser.v
@@ -1,86 +1,49 @@
 From Pollux Require Import Prelude.
 From Pollux.parse Require Import Util.
 From Pollux.parse Require Import Input.
+From Pollux.parse Require Import Failure.
 
 From Corelib.Program Require Import Basics Tactics.
 From Stdlib.Program Require Import Program.
-From Equations Require Import Equations.
 
 Module Parsers (InputModule : AbstractInput).
-  Section Parsers.
-    Import InputModule.
+  Module Failure := Failures(InputModule).
+  Import InputModule.
 
+  Section Results.
     Context `{EqDecision Input}.
 
-    Inductive FailureLevel :=
-    | Fatal
-    | Recoverable.
+    Inductive Result {X : Type} :=
+    | Success (result : X) (remaining : Input)
+    | Failure (level : Failure.Level) (data : Failure.Data).
+    Arguments Result X : clear implicits.
 
-    (* Record information about when a parse / serialize fails *)
-    Inductive FailureData :=
-    | mkFailureData (msg : string) (remaining : Input) (next : option FailureData).
-
-    Definition getFailureMsg (data : FailureData) : string :=
-      match data with
-      | mkFailureData msg _ _ => msg
-      end.
-
-    Definition getFailureRemaining (data : FailureData) : Input :=
-      match data with
-      | mkFailureData _ remaining _ => remaining
-      end.
-
-    Definition getFailureNext (data : FailureData) : option FailureData :=
-      match data with
-      | mkFailureData _ _ next => next
-      end.
-
-    (* Add more failure data to the end of the current chain of failures *)
-    Fixpoint ConcatFailure (self other : FailureData) : FailureData :=
-      match self with
-      | mkFailureData msg remaining next =>
-          match next with
-          | None => mkFailureData msg remaining (Some other)
-          | Some next_val => mkFailureData msg remaining (Some (ConcatFailure next_val other))
-          end
-      end.
-
-    (** I'll use the failure for the serializers too, but interpret "remaining" as "output". *)
-    
-    Inductive ParseResult {R : Type} :=
-    | ParseSuccess (result : R) (remaining : Input)
-    | ParseFailure (level : FailureLevel) (data : FailureData).
-    
-    Arguments ParseResult R : clear implicits.
-
-    (**
-     FUNCTIONS ON PARSE RESULTS
-     *)
+    (** FUNCTIONS ON PARSE RESULTS *)
 
     (* If Remaining is the same as the input, then parser is "uncommitted",
      so combinators like Or or ZeroOrMore can try alternatives. *)
-    Definition Remaining {R : Type} (pr : ParseResult R) : Input :=
+    Definition Remaining {X : Type} (pr : Result X) : Input :=
       match pr with
-      | ParseSuccess _ rem
-      | ParseFailure _ (mkFailureData _ rem _) => rem
+      | Success _ rem
+      | Failure _ (Failure.mkData _ rem _) => rem
       end.
     
-    Definition IsFailure {R : Type} (pr : ParseResult R) : bool :=
+    Definition IsFailure {X : Type} (pr : Result X) : bool :=
       match pr with
-      | ParseFailure _ _ => true
+      | Failure _ _ => true
       | _ => false
       end.
 
-    Definition IsFatalFailure {R : Type} (pr : ParseResult R) : bool :=
+    Definition IsFatalFailure {X : Type} (pr : Result X) : bool :=
       match pr with
-      | ParseFailure Fatal _ => true
+      | Failure Failure.Fatal _ => true
       | _ => false
       end.
 
-    Definition IsFailureProp {R : Type} (pr : ParseResult R) : Prop :=
+    Definition IsFailureProp {X : Type} (pr : Result X) : Prop :=
       match pr with
-      | ParseSuccess _ _ => False
-      | ParseFailure _ _ => True
+      | Success _ _ => False
+      | Failure _ _ => True
       end.
 
     (* This function basically lets us change the parameterized type of a parse failure. This is useful
@@ -90,459 +53,153 @@ Module Parsers (InputModule : AbstractInput).
      the same parse failure but with the correct type. It takes a proof term as input since this
      only makes sense for failures. Successes with have something of type R in them, which we can't
      convert to a U. *)
-    Definition PropagateFailure {R : Type} {U : Type} (pr : ParseResult R) (pf : IsFailureProp pr) :
-      ParseResult U.
+    Definition Propagate {A B : Type} (pr : Result A) (pf : IsFailureProp pr) :
+      Result B.
     Proof.
       destruct pr.
       - destruct pf.
-      - apply ParseFailure; assumption.
+      - apply Failure; assumption.
     Defined.
 
-    Definition IsSuccessProp {R : Type} (pr : ParseResult R) : Prop :=
+    Definition IsSuccessProp {X : Type} (pr : Result X) : Prop :=
       match pr with
-      | ParseSuccess _ _ => True
-      | ParseFailure _ _ => False
+      | Success _ _ => True
+      | Failure _ _ => False
       end.
 
     (* Similarly to PropagateFailure, this function only works on a ParseSuccess and lets us unwrap it.
      Honestly, both of these could be done inline whenever needed, but I like learning more about how
      to handle these in Rocq. I don't know what extraction would do to these. *)
-    Definition Extract {R : Type} (pr : ParseResult R) (pf : IsSuccessProp pr) : R * Input. 
+    Definition Extract {X : Type} (pr : Result X) (pf : IsSuccessProp pr) : X * Input. 
     Proof.
       destruct pr.
       - split; assumption.
       - destruct pf.
     Defined.
 
-    Definition ResultMap {R : Type} {R' : Type} (pr : ParseResult R) (f : R -> R') : ParseResult R' :=
+    Definition ResultMap {X Y : Type} (pr : Result X) (f : X -> Y) : Result Y :=
       match pr with
-      | ParseSuccess result remaining => ParseSuccess (f result) remaining
-      | ParseFailure lvl data => ParseFailure lvl data
+      | Success result remaining => Success (f result) remaining
+      | Failure lvl data => Failure lvl data
       end.
 
-    Definition MapRecoverableError {R : Type} (pr : ParseResult R) (f : FailureData -> FailureData) :
-      ParseResult R :=
+    Definition MapRecoverableError {X : Type} (pr : Result X) (f : Failure.Data -> Failure.Data) :
+      Result X :=
       match pr with
-      | ParseFailure Recoverable data => ParseFailure Recoverable (f data)
+      | Failure Failure.Recoverable data => Failure Failure.Recoverable (f data)
       | _ => pr
       end.
 
-    Definition NeedsAlternative {R : Type} (pr : ParseResult R) (input : Input) : bool :=
+    Definition NeedsAlternative {X : Type} (pr : Result X) (input : Input) : bool :=
       match pr with
-      | ParseFailure Recoverable (mkFailureData _ rem _) => if rem == input then true else false
+      | Failure Failure.Recoverable (Failure.mkData _ rem _) => if rem == input then true else false
       | _ => false
       end.
 
-    (** SERIALIZER RESULTS *)
+    End Results.
+    Arguments Result X : clear implicits.
 
-    (* Use Output type for serializers *)
-    Definition Output := Input.
+    Section Def.
+      (** Parser Definition *)
 
-    Inductive SerializeResult :=
-    | SerialSuccess (out : Output)
-    | SerialFailure (level : FailureLevel) (data : FailureData).
+      (* A parser is a total function from a position to a parse result *)
+      Definition Parser (X : Type) := Input -> Result X.
 
-    (** FUNCTIONS ON SERIALIZER RESULTS *)
+      Definition IsRemaining (input remaining : Input) : Prop :=
+        Length remaining <= Length input /\ Drop input (Length input - Length remaining) = remaining.
 
-    Definition Out (sr : SerializeResult) : Output := 
-      match sr with
-      | SerialSuccess out
-      | SerialFailure _ (mkFailureData _ out _) => out
-      end.
+      Lemma IsRemainingTrans (input remaining1 remaining2 : Input) :
+        IsRemaining input remaining1 -> IsRemaining remaining1 remaining2 -> IsRemaining input remaining2.
+      Proof using Type.
+        intros [H1_len H1_drop] [H2_len H2_drop].
+        unfold IsRemaining.
+        split.
+        - apply Nat.le_trans with (Length remaining1); assumption.
+        - rewrite <- H2_drop at 2. 
+          rewrite <- H1_drop at 1.
+          rewrite <- DropDrop.
+          * rewrite Nat.add_sub_assoc; last assumption.
+            rewrite Nat.sub_add; last assumption.
+            reflexivity.
+          * lia.
+          * lia.
+      Qed.
 
-    Definition IsSerialFailure (sr : SerializeResult) : bool :=
-      match sr with
-      | SerialFailure _ _ => true
-      | _ => false
-      end.
-    
-    Definition IsSerialFatalFailure (sr : SerializeResult) : bool :=
-      match sr with
-      | SerialFailure Fatal _ => true
-      | _ => false
-      end.
+    End Def.
 
-    Definition IsSerialFailureProp (sr : SerializeResult) : Prop :=
-      match sr with
-      | SerialSuccess _ => False
-      | SerialFailure _ _ => True
-      end.
-    
-    (* PropagateSerialFailure function not needed since SerializeResults are parameterized. *)
+    Section Combinators.
+      Context `{EqDecision Input}.
 
-    Definition IsSerialSuccessProp (sr : SerializeResult) : Prop :=
-      match sr with
-      | SerialSuccess _ => True
-      | SerialFailure _ _ => False
-      end.
+      (* This parser does not consume any input and returns the given value *)
+      Definition SucceedWith {X : Type} (result : X) : Parser X :=
+        fun inp => Success result inp.
 
-    (**
-     Parser Definition
+      (* A parser that always succeeds, consumes nothing and returns () *)
+      Definition Epsilon : (Parser unit) := SucceedWith tt.
 
-     This are missing Dafny variance specifiers. I don't know how big of a problem this will be
-     *)
+      (* A parser that does not consume any input and returns the given failure *)
+      Definition FailWith {X : Type} (message : string) (level : Failure.Level) : Parser X :=
+        fun inp => Failure level $ Failure.mkData message inp None.
 
-    (* A parser is a total function from a position to a parse result *)
-    Definition Parser R : Type := Input -> ParseResult R.
-
-    (* A parser selector is a function that, given a name that exists,
-     returns a parser associated to this name *)
-    Definition ParserSelector R : Type := string -> ParseResult R.
-
-    (** Serializer Definition *)
-
-    Definition Serializer (R : Type) (wf : R -> Prop) := R -> SerializeResult. 
-
-    (**
-     Misc Utilities and Definitions
-     *)
-    Definition IsRemaining (input remaining : Input) : Prop :=
-      Length remaining <= Length input /\ Drop input (Length input - Length remaining) = remaining.
-
-    Lemma IsRemainingTrans (input remaining1 remaining2 : Input) :
-      IsRemaining input remaining1 -> IsRemaining remaining1 remaining2 -> IsRemaining input remaining2.
-    Proof using Type.
-      intros [H1_len H1_drop] [H2_len H2_drop].
-      unfold IsRemaining.
-      split.
-      - apply Nat.le_trans with (Length remaining1); assumption.
-      - rewrite <- H2_drop at 2. 
-        rewrite <- H1_drop at 1.
-        rewrite <- DropDrop.
-        * rewrite Nat.add_sub_assoc; last assumption.
-          rewrite Nat.sub_add; last assumption.
-          reflexivity.
-        * lia.
-        * lia.
-    Qed.
-
-    (** TOP LEVEL CORRECTNESS DEFINITION *)
-    Definition ParseOk''' {R : Type} {wf : R -> Prop}
-      (par : Parser R) (ser : Serializer R wf) (x : R) (enc rest : Input) :=
-      wf x -> ser x = SerialSuccess enc -> par (App enc rest) = ParseSuccess x rest.
-
-    Definition ParseOk'' {R : Type} {wf : R -> Prop}
-      (par : Parser R) (ser : Serializer R wf) (x : R) (enc : Input) :=
-      forall (rest : Input), ParseOk''' par ser x enc rest.
-
-    Definition ParseOk' {R : Type} {wf : R -> Prop} (par : Parser R) (ser : Serializer R wf) (x : R) :=
-      forall (enc : Input), ParseOk'' par ser x enc.
-
-    Definition ParseOk {R : Type} {wf : R -> Prop} (par : Parser R) (ser : Serializer R wf) :=
-      forall (x : R), ParseOk' par ser x.
-
-    (**
-     COMBINATORS
-     *)
-
-    (* This parser does not consume any input and returns the given value *)
-    Definition ParseSucceedWith {R : Type} (result : R) : Parser R :=
-      (fun inp => ParseSuccess result inp).
-
-    Definition serial_trivial_wf {R : Type} : R -> Prop := fun _ => True.
-
-    Definition SerialSucceedWith {R : Type} : Serializer R serial_trivial_wf :=
-      (fun inp => SerialSuccess Input_default).
-
-    Lemma SucceedCorrect {R : Type} (r : R) :
-      ParseOk' (ParseSucceedWith r) SerialSucceedWith r.
-    Proof using Type.
-      intros enc rest wf_ok. 
-      unfold SerialSucceedWith.
-      intros Hser_ok. inversion Hser_ok as [Henc].
-      unfold ParseSucceedWith.
-      rewrite App_nil_l.
-      reflexivity.
-    Qed.
-
-    (* A parser that always succeeds, consumes nothing and returns () *)
-    Definition ParseEpsilon : (Parser unit) := ParseSucceedWith tt.
-
-    Definition SerialEpsilon : (Serializer unit serial_trivial_wf) := SerialSucceedWith.
-
-    (* While we couldn't do this for any type (see SucceedCorrect above), we CAN do it with unit
-       since we know statically that there is only one member of type unit, (). *)
-    Lemma EpsilonCorrect : ParseOk ParseEpsilon SerialEpsilon.
-    Proof using Type.
-      intros x enc rest Hwf Hser_ok.
-      inversion Hser_ok as [Hdefault].
-      subst.
-      unfold ParseEpsilon.
-      unfold ParseSucceedWith.
-      rewrite App_nil_l.
-      destruct x.
-      reflexivity.
-    Qed.
-
-    (* A parser that does not consume any input and returns the given failure *)
-    Definition ParseFailWith {R : Type} (message : string) (level : FailureLevel) : Parser R :=
-      fun inp => ParseFailure level $ mkFailureData message inp None.
-
-    Definition SerialFailWith {R : Type} (message : string) (level : FailureLevel) :
-      Serializer R serial_trivial_wf :=
-        fun inp => SerialFailure level $ mkFailureData message Input_default None.
-
-    (* WARN I don't think a connecting lemma here is possible. *)
-
-    (* A parser that always returns the given result *)
-    Definition ParseResultWith {R : Type} (result : ParseResult R) : Parser R :=
-      fun inp => result.
-
-    Definition SerialResultWith {R : Type} (result : SerializeResult) : Serializer R serial_trivial_wf :=
-      fun inp => result.
-
-    (* WARN I don't think a connecting lemma here is possible. *)
+      (* A parser that always returns the given result *)
+      Definition ResultWith {X : Type} (result : Result X) : Parser X :=
+        fun inp => result.
 
     (* A parser that fails if the string has not been entirely consumed *)
-    Definition ParseEndOfInput : Parser unit :=
-      fun inp => if Length inp == 0 then
-                ParseSuccess () inp
-              else
-                ParseFailure Recoverable
-                  (mkFailureData "expected end of input" inp None).
-
-    (* WARN I also don't there is a corresponding serializer combinator here. *)
-
-    Definition SerialBlob : Serializer Output serial_trivial_wf :=
-      fun b => SerialSuccess b.
+      Definition EndOfInput : Parser unit :=
+        fun inp => if Length inp == 0 then
+                  Success () inp
+                else
+                  Failure Failure.Recoverable
+                    (Failure.mkData "expected end of input" inp None).
 
     (* A parser that fails if the left parser fails. If the left parser succeeds, provides its
      result and the remaining sequence to the right parser generator. *)
-    Definition ParseBind {L R : Type} (left : Parser L) (right : L -> Parser R) : Parser R :=
+    Definition Bind {L R : Type} (left : Parser L) (right : L -> Parser R) : Parser R :=
       fun inp =>
         match left inp with
-        | ParseSuccess leftResult remaining => right leftResult remaining
-        | ParseFailure level data => ParseFailure level data
+        | Success leftResult remaining => right leftResult remaining
+        | Failure level data => Failure level data
         end.
-
-    Definition Bind_wf {L R : Type} {wfl : L -> Prop} {wfr : R -> Prop}
-      (tag : R -> L) (left : R -> Serializer L wfl) (right : Serializer R wfr) : R -> Prop :=
-      fun r => wfl (tag r) /\ wfr r.
-
-    Definition SerialBind {L R : Type} {wfl : L -> Prop} {wfr : R -> Prop} 
-      (tag : R -> L) (left : forall r, Serializer L (fun l => l = tag r /\ wfl l)) (right : Serializer R wfr) :
-      Serializer R (@Bind_wf L R wfl wfr tag left right) := 
-      fun r =>
-        match left r (tag r) with
-        | SerialSuccess l_enc => match right r with
-                                | SerialSuccess r_enc => SerialSuccess (App l_enc r_enc)
-                                | SerialFailure lvl data as f => f
-                                end
-        | SerialFailure lvl data as f => f
-        end.
-
-    Lemma BindCorrect {L R : Type} {wfl : L -> Prop} {wfr : R -> Prop}
-      (lp : Parser L) (ls : R -> Serializer L wfl)
-      (rp : L -> Parser R) (rs : Serializer R wfr) (tag : R -> L) :
-      forall r, ParseOk lp (ls r) -> ParseOk (rp (tag r)) rs ->
-      ParseOk' (ParseBind lp rp) (SerialBind tag ls rs) r.
-    Proof using Type.
-      intros x Hleft_ok Hright_ok enc rest wf_ok.
-      unfold SerialBind.
-      destruct (ls x (tag x)) as [l_enc|] eqn:Hleft; last discriminate.
-      destruct (rs x) as [r_enc|] eqn:Hright; last discriminate.
-      intro Hser_ok. inversion Hser_ok as [Henc].
-      rewrite App_assoc.
-      unfold ParseBind.
-      destruct wf_ok as [wfl_ok wfr_ok].
-      pose proof Hleft_ok (tag x) l_enc (App r_enc rest) wfl_ok Hleft as Hl_ret.
-      rewrite Hl_ret.
-      pose proof Hright_ok x r_enc rest wfr_ok Hright as Hr_ret.
-      assumption.
-    Qed.
 
     (* A parser that fails if the left parser fails. If the left parser
      succeeds, provides its result to the right parser generator and returns its
      result applied to the remaining input *)
-    Definition ParseBindSucceeds {L R : Type} (left : Parser L) (right : L -> Input -> Parser R) : Parser R :=
+    Definition BindSucceeds {L R : Type} (left : Parser L) (right : L -> Input -> Parser R) : Parser R :=
       fun inp =>
         match left inp with
-        | ParseSuccess leftResult remaining => right leftResult remaining remaining
-        | ParseFailure level data => ParseFailure level data
+        | Success leftResult remaining => right leftResult remaining remaining
+        | Failure level data => Failure level data
         end.
-
-    Definition BindSucceeds_wf {L R : Type} {wfl : L -> Prop} {wfr : R -> Prop}
-      (tag : R -> L) (left : R -> Output -> Serializer L wfl) (right : Serializer R wfr) : R -> Prop :=
-      fun r => wfl (tag r) /\ wfr r.
-
-    (* This is tricky since technically ParseBindSucceeds isn't limited to only
-    inspecting the encoding of the right serializer (could use things like the
-    lookahead parser) so the correctness theorem will have to ensure that both
-    get the same encoding. *)
-    Definition SerialBindSucceeds {L R : Type} {wfl : L -> Prop} {wfr : R -> Prop}  
-      (tag : R -> L) (left : R -> Output -> Serializer L wfl) (right : Serializer R wfr) :
-      Serializer R (BindSucceeds_wf tag left right) := 
-      fun r =>
-        match right r with
-        | SerialSuccess r_enc => match left r r_enc (tag r) with
-                                | SerialSuccess l_enc => SerialSuccess (App l_enc r_enc)
-                                | SerialFailure lvl data as f => f
-                                end
-        | SerialFailure lvl data as f => f
-        end.
-
-    Definition BindSucceedsRightOk {R L : Type} {wfr : R -> Prop}
-      (rp : L -> Input -> Parser R) (rs : Serializer R wfr) (tag : R -> L) : Prop := 
-      forall (r : R) (r_enc rest : Input), ParseOk''' (rp (tag r) (App r_enc rest)) rs r r_enc rest.
-
-    Definition BindSucceedsLeftOk {R L : Type} {wfl : L -> Prop}
-      (lp : Parser L) (ls : R -> Output -> Serializer L wfl) (tag : R -> L) : Prop :=
-      forall (r : R) (l_enc r_enc rest : Input), ParseOk''' lp (ls r r_enc) (tag r) l_enc (App r_enc rest).
-
-    Lemma BindSucceedsCorrect {L R : Type} {wfl : L -> Prop} {wfr : R -> Prop}
-      (lp : Parser L) (ls : R -> Output -> Serializer L wfl)
-      (rp : L -> Input -> Parser R) (rs : Serializer R wfr) (tag : R -> L) :
-      BindSucceedsRightOk rp rs tag -> BindSucceedsLeftOk lp ls tag ->
-      ParseOk (ParseBindSucceeds lp rp) (SerialBindSucceeds tag ls rs).
-    Proof using Type.
-      intros Hright_ok Hleft_ok x enc rest wf_ok.
-      unfold SerialBindSucceeds.
-      destruct (rs x) as [r_enc|] eqn:Hright; last discriminate.
-      destruct (ls x r_enc (tag x)) as [l_enc|] eqn:Hleft; last discriminate.
-      intros Hser_ok. inversion Hser_ok as [Henc].
-      destruct wf_ok as [wfl_ok wfr_ok].
-      rewrite App_assoc.
-      unfold ParseBindSucceeds.
-      pose proof Hleft_ok x l_enc r_enc rest as Hlp.
-      pose proof wfl_ok as wfl_ok'.
-      apply Hlp in wfl_ok' as _, Hleft as Hl_ret; try assumption.
-      rewrite Hl_ret.
-      pose proof Hright_ok x r_enc rest as Hrp.
-      pose proof wfr_ok as wfr_ok'.
-      apply Hrp in wfr_ok' as _, Hright as Hr_ret; try assumption.
-    Qed.
 
     (* Given a left parser and a parser generator based on the output of the left parser,
      returns the result of the right parser applied on the original input. *)
-    Definition ParseBindResult {L R : Type} (left : Parser L) (right : ParseResult L -> Input -> Parser R) :
+    Definition BindResult {L R : Type} (left : Parser L) (right : Result L -> Input -> Parser R) :
       Parser R :=
       fun inp =>
         right (left inp) inp inp.
 
-    Definition BindResult_wf {L R : Type} {wfl : L -> Prop} {wfr : R -> Prop}
-      (tag : R -> L) (left : SerializeResult -> Output -> Serializer L wfl) (right : Serializer R wfr) :
-      R -> Prop :=
-      fun r => wfl (tag r) /\ wfr r.
-
-    Definition SerialBindResult {L R : Type} {wfl : L -> Prop} {wfr : R -> Prop}
-      (tag : R -> L) (left : SerializeResult -> Output -> Serializer L wfl) (right : Serializer R wfr) :
-      Serializer R (BindResult_wf tag left right) :=
-      fun r =>
-        let r_ret := right r in
-        left r_ret (Out r_ret) (tag r).
-
-    Definition BindResultLeftOk {L R : Type} {wfl : L -> Prop} {wfr : R -> Prop}
-      (lp : Parser L) (ls : SerializeResult -> Output -> Serializer L wfl)
-      (rs : Serializer R wfr) (tag : R -> L): Prop :=
-      forall (r : R), ParseOk' lp (ls (rs r) (Out $ rs r)) (tag r).
-
-    Definition BindResultRightOk {L R : Type} {wfr : R -> Prop}
-      (rp : ParseResult L -> Input -> Parser R) (rs : Serializer R wfr)
-      (lp : Parser L) (tag : R -> L) : Prop :=
-      forall (r : R) (l_enc r_enc rest: Input),
-      let enc := (App (App l_enc r_enc) rest) in
-      ParseOk''' (rp (lp enc) enc) rs r r_enc rest.
-
-    Lemma BindResultCorrect {L R : Type} {wfl : L -> Prop} {wfr : R -> Prop}
-      (lp : Parser L) (ls : SerializeResult -> Output -> Serializer L wfl)
-      (rp : ParseResult L -> Input -> Parser R) (rs : Serializer R wfr) (tag : R -> L) :
-      BindResultLeftOk lp ls rs tag -> BindResultRightOk rp rs lp tag ->
-      ParseOk (ParseBindResult lp rp) (SerialBindResult tag ls rs).
-    Proof using Type.
-      unfold ParseOk, ParseOk', ParseOk'', ParseOk'''.
-      intros Hleft_ok Hright_ok x enc rest wf_ok.
-      unfold SerialBindResult.
-      destruct (rs x) as [r_enc|] eqn:Hright.
-      - simpl. symmetry in Hright.
-        intro Hls. unfold BindResult_wf in wf_ok.
-        destruct wf_ok as [wfl_ok wfr_ok].
-        pose proof Hright as Hright'.
-        pose proof Hleft_ok x enc rest as Hlp. 
-        rewrite <- Hright in Hlp. simpl in Hlp.
-        pose proof wfl_ok as wfl_ok'.
-        apply Hlp in wfl_ok' as _, Hls as Hl_ret; try assumption.
-        unfold ParseBindResult.
-        rewrite Hl_ret.
-
-        unfold BindResultRightOk, ParseOk', ParseOk'', ParseOk''' in Hright_ok.
-        pose proof Hright_ok x enc r_enc rest as Hr.
-        pose proof wfr_ok as wfr_ok'.
-        symmetry in Hright'.
-        apply Hr in wfr_ok' as _, Hright' as Hr_ret; try assumption.
-        (* rewrite Hl_ret in Hr_ret. *)
-    Abort.
-
     (* Apply two parser consecutively. If both succeed, return the pair of both results *)
-    Definition ParseConcat {L R : Type} (left : Parser L) (right : Parser R) : Parser (L * R) :=
+    Definition Concat {L R : Type} (left : Parser L) (right : Parser R) : Parser (L * R) :=
       fun inp =>
         match left inp with
-        | ParseSuccess ll lrem => match right lrem with
-                                 | ParseSuccess rr rrem => ParseSuccess (ll, rr) rrem
-                                 | ParseFailure lvl data as p => PropagateFailure p I
+        | Success ll lrem => match right lrem with
+                                 | Success rr rrem => Success (ll, rr) rrem
+                                 | Failure lvl data as p => Propagate p I
                                  end
-        | ParseFailure lvl data as p => PropagateFailure p I
+        | Failure lvl data as p => Propagate p I
         end.
-
-    Definition Concat_wf {L R : Type} (wfl : L -> Prop) (wfr : R -> Prop) : (L * R) -> Prop :=
-      fun lr => let (l, r) := lr in wfl l /\ wfr r.
-
-    Definition SerialConcat {L R : Type} {wfl : L -> Prop} {wfr : R -> Prop}
-      (left : Serializer L wfl) (right : Serializer R wfr) : Serializer (L * R) (Concat_wf wfl wfr) :=
-      fun inp =>
-        let (l, r) := inp in 
-        match left l, right r with
-        | SerialSuccess l_enc, SerialSuccess r_enc => SerialSuccess (App l_enc r_enc)
-        | SerialFailure level data, _
-        | _, SerialFailure level data => SerialFailure level data
-        end.
-
-    Lemma SerialConcatInversion : forall {A B : Type} {wf__a : A -> Prop} {wf__b : B -> Prop}
-                                      (ser__a : Serializer A wf__a) (ser__b : Serializer B wf__b)
-                                      (a : A) (b : B) (enc : Output),
-      SerialConcat ser__a ser__b (a, b) = SerialSuccess enc <->
-                                        exists (enc__a enc__b : Output),
-                                          ser__a a = SerialSuccess enc__a /\
-                                          ser__b b = SerialSuccess enc__b /\
-                                          enc = App enc__a enc__b.
-    Proof using Type.
-      intros. split.
-      - unfold SerialConcat.
-        destruct (ser__a a) as [out__a |] eqn:Ha; last discriminate.
-        destruct (ser__b b) as [out__b |] eqn:Hb; last discriminate.
-        intro H. inversion H as [Henc]. clear H.
-        exists out__a, out__b. repeat (split; first reflexivity); reflexivity.
-      - intros (out__a & out__b & Ha & Hb & Henc). unfold SerialConcat.
-        rewrite Ha. rewrite Hb.
-        subst. reflexivity.
-    Qed.
-
-    Theorem ConcatCorrect {L R : Type} {wfl : L -> Prop} {wfr : R -> Prop}
-      (lp : Parser L) (ls : Serializer L wfl)
-      (rp : Parser R) (rs : Serializer R wfr) :
-      ParseOk lp ls -> ParseOk rp rs -> ParseOk (ParseConcat lp rp) (SerialConcat ls rs).
-    Proof using Type.
-      intros Hleft_ok Hright_ok.
-      intros [l r] enc rest [Hl_wf Hr_wf] Hconcat.
-      apply SerialConcatInversion in Hconcat.
-      destruct Hconcat as (enc__l & enc__r & Hl & Hr & Henc).
-      subst. rewrite App_assoc.
-      apply (Hleft_ok _ _ (App enc__r rest)) in Hl; last assumption.
-      apply (Hright_ok _ _ rest) in Hr; last assumption.
-      unfold ParseConcat.
-      rewrite Hl. rewrite Hr.
-      reflexivity.
-    Qed.
 
     (* Apply two consecutive parsers consecutively. If both succeed, apply the mapper to the results
      and return it *)
     Definition ConcatMap {L R T : Type} (left : Parser L) (right : Parser R) (mapper : L -> R -> T) : Parser T :=
       fun inp =>
         match left inp with
-        | ParseSuccess ll lrem => match right lrem with
-                                 | ParseSuccess rr rrem => ParseSuccess (mapper ll rr) rrem
-                                 | ParseFailure lvl data as p => PropagateFailure p I
-                                 end
-        | ParseFailure lvl data as p => PropagateFailure p I
+        | Success ll lrem => match right lrem with
+                            | Success rr rrem => Success (mapper ll rr) rrem
+                            | Failure lvl data as p => Propagate p I
+                            end
+        | Failure lvl data as p => Propagate p I
         end.
 
     (* Return only the result of the right parser if the two parsers match *)
@@ -553,208 +210,35 @@ Module Parsers (InputModule : AbstractInput).
     Definition ConcatKeepLeft {L R : Type} (left : Parser L) (right : Parser R) : Parser L :=
       ConcatMap left right (fun l r => l).
     
-    Definition SerialBind' {L R : Type} {wfl : L -> Prop} {wfr : R -> Prop}
-      (tag : R -> L) (left : Serializer L wfl) (right : Serializer R wfr) :
-      Serializer R (fun r => wfl (tag r) /\ wfr r) :=
-      fun r => SerialConcat left right (tag r, r).
-
-    Lemma BindCorrect' {L R : Type} {wfl : L -> Prop} {wfr : R -> Prop}
-      (lp : Parser L) (ls : Serializer L wfl)
-      (rp : L -> Parser R) (rs : Serializer R wfr) (tag : R -> L) :
-      forall r, ParseOk lp ls -> ParseOk' (rp (tag r)) rs r -> ParseOk' (ParseBind lp rp) (SerialBind' tag ls rs) r.
-    Proof using Type.
-      intros r Hleft_ok Hright_ok enc rest [wfl_ok wfr_ok] Hbind.
-      apply SerialConcatInversion in Hbind.
-      destruct Hbind as (enc__l & enc__r & Hl_ok & Hr_ok & Henc).
-      rewrite Henc. rewrite App_assoc.
-      unfold ParseBind.
-      apply (Hleft_ok _ _ (App enc__r rest)) in Hl_ok; last assumption.
-      rewrite Hl_ok.
-      apply (Hright_ok _ rest) in Hr_ok; assumption.
-    Qed.
-
     (* Limit the underlying parser to only access the first N tokens in the input. *)
-    Definition ParseLimit {R : Type} (underlying : Parser R) (n : nat) : Parser R :=
+    Definition Limit {X : Type} (underlying : Parser X) (n : nat) : Parser X :=
       fun inp => match underlying (Slice inp 0 n) with
-              | ParseSuccess r rem => ParseSuccess r (App rem (Drop inp n))
-              | ParseFailure lvl data as f => f
+              | Success r rem => Success r (App rem (Drop inp n))
+              | Failure lvl data as f => f
               end.
 
-    (* This formulation is only useful for the proof. *)
-    Definition SerialLimit {R : Type} {wfr : R -> Prop} (underlying : Serializer R wfr) (len : R -> nat) :
-      Serializer R wfr := underlying.
-
-    Definition ParseLen {R : Type} (len : Parser nat) (underlying : Parser R) : Parser R :=
-      ParseBind len (fun l => ParseLimit underlying l).
-
-    Definition SerialLen {R : Type} {wfr : R -> Prop} {wfn : nat -> Prop} (len : R -> nat)
-      (ser_len : Serializer nat wfn) (underlying : Serializer R wfr) : Serializer R (fun r => wfn (len r) /\ wfr r) :=
-      SerialBind' (len) ser_len (SerialLimit underlying len).
-
-    Definition SerialLen'_wf {R : Type} {wfr : R -> Prop} {wfn : nat -> Prop}
-      (s__len : Serializer nat wfn) (s__r : Serializer R wfr) : R -> Prop :=
-      fun r => match s__r r with
-            | SerialSuccess enc__r => match s__len (Length enc__r) with
-                                  | SerialSuccess enc__len => wfn (Length enc__r) /\ wfr r
-                                  | SerialFailure _ _ => True
-                                  end
-            | SerialFailure _ _ => True
-            end.
-    
-    Definition SerialLen' {R : Type} {wfr : R -> Prop} {wfn : nat -> Prop}
-      (ser_len : Serializer nat wfn) (underlying : Serializer R wfr) :
-      Serializer R $ SerialLen'_wf ser_len underlying :=
-      fun r => match underlying r with
-            | SerialSuccess enc => match ser_len (Length enc) with
-                                  | SerialSuccess len_enc => SerialSuccess (App len_enc enc)
-                                  | SerialFailure lvl data as f => f
-                                  end
-            | SerialFailure lvl data as f => f
-            end.
-
-    (* Relax the rest requirement, since the Limit parser will ensure rest = [] *)
-    Definition LimitParseOk {R : Type} {wf : R -> Prop} (ser : Serializer R wf) (par : Parser R) := 
-      forall x enc,
-      wf x -> ser x = SerialSuccess enc -> par enc = ParseSuccess x Input_default.
-
-    Definition LenOk {R : Type} {wf : R -> Prop} (ser : Serializer R wf) (len : R -> nat) (r : R) :=
-      forall enc, ser r = SerialSuccess enc -> len r = Length enc.
-
-    Lemma LimitCorrect {R : Type} {wf : R -> Prop} (len : R -> nat)
-      (underlying__ser : Serializer R wf) (underlying__par : Parser R) (r : R) :
-      LimitParseOk underlying__ser underlying__par ->
-      LenOk underlying__ser len r ->
-      ParseOk' (ParseLimit underlying__par (len r)) (SerialLimit underlying__ser len) r.
-    Proof using Type.
-      intros Hlim_ok Hlen_ok.
-      intros enc rest Hwf.
-      unfold SerialLimit, ParseLimit.
-      intros Hser.
-      unfold LenOk in Hlen_ok.
-      specialize (Hlen_ok enc Hser).
-      rewrite Hlen_ok.
-      rewrite Slice_App.
-      specialize (Hlim_ok r enc Hwf Hser).
-      rewrite Hlim_ok.
-      rewrite Drop_App, App_nil_l.
-      reflexivity.
-    Qed.
-
-    Lemma LenCorrect {R : Type} {wfr : R -> Prop} {wfn : nat -> Prop}
-      (ser__len : Serializer nat wfn) (par__len : Parser nat) (len : R -> nat)
-      (ser__r : Serializer R wfr) (par__r : Parser R) (r : R) :
-      ParseOk par__len ser__len ->
-      LimitParseOk ser__r par__r ->
-      LenOk ser__r len r ->
-      ParseOk' (ParseLen par__len par__r) (SerialLen len ser__len ser__r) r.
-    Proof using Type.
-      intros Hnat_ok Hlim_ok Hlen_ok.
-      unfold ParseLen, SerialLen.
-      apply BindCorrect'; first assumption.
-      apply LimitCorrect; assumption.
-    Qed.
-
-    Definition LimitParseOkWeak {R : Type} {wf : R -> Prop} (ser : Serializer R wf) (par : Parser R)
-      (x : R) := 
-      forall enc,
-      wf x -> ser x = SerialSuccess enc -> par enc = ParseSuccess x Input_default.
-
-    Lemma LenCorrect'Weakened {R : Type} {wfr : R -> Prop} {wfn : nat -> Prop}
-      (ser__len : Serializer nat wfn) (par__len : Parser nat)
-      (ser__r : Serializer R wfr) (par__r : Parser R) (r : R) :
-      ParseOk par__len ser__len ->
-      LimitParseOkWeak ser__r par__r r ->
-      ParseOk' (ParseLen par__len par__r) (SerialLen' ser__len ser__r) r.
-    Proof using Type.
-      intros Hnat_ok Hlim_ok.
-      intros enc' rest Hwf.
-      unfold ParseLen, SerialLen', ParseOk'''.
-      destruct (ser__r r) as [enc__r |] eqn:Hser__r; last discriminate.
-      destruct (ser__len (Length enc__r)) as [enc__len |] eqn:Hser__len; last discriminate.
-      unfold SerialLen'_wf in Hwf.
-      rewrite Hser__r in Hwf.
-      rewrite Hser__len in Hwf.
-      destruct Hwf as [Hwf__len Hwf__r].
-      intros Henc. inversion Henc as [Henc__r].
-      unfold ParseBind.
-      rewrite App_assoc.
-      specialize (Hnat_ok (Length enc__r) enc__len (App enc__r rest) Hwf__len Hser__len); rewrite Hnat_ok.
-      unfold ParseLimit.
-      rewrite Slice_App.
-      specialize (Hlim_ok enc__r Hwf__r Hser__r); rewrite Hlim_ok.
-      rewrite App_nil_l, Drop_App.
-      reflexivity.
-    Qed.
-      
-    Lemma LenCorrect' {R : Type} {wfr : R -> Prop} {wfn : nat -> Prop}
-      (ser__len : Serializer nat wfn) (par__len : Parser nat)
-      (ser__r : Serializer R wfr) (par__r : Parser R) :
-      ParseOk par__len ser__len ->
-      LimitParseOk ser__r par__r ->
-      ParseOk (ParseLen par__len par__r) (SerialLen' ser__len ser__r).
-    Proof using Type.
-      intros Hnat_ok Hlim_ok.
-      intros r enc rest Hwf.
-      unfold ParseLen, SerialLen'.
-      destruct (ser__r r) as [enc__r |] eqn:Hser__r; last discriminate.
-      destruct (ser__len (Length enc__r)) as [enc__len |] eqn:Hser__len; last discriminate.
-      unfold SerialLen'_wf in Hwf.
-      rewrite Hser__r in Hwf.
-      rewrite Hser__len in Hwf.
-      destruct Hwf as [Hwf__len Hwf__r].
-      intros Henc. inversion Henc.
-      unfold ParseBind.
-      rewrite App_assoc.
-      specialize (Hnat_ok (Length enc__r) enc__len (App enc__r rest) Hwf__len Hser__len); rewrite Hnat_ok.
-      unfold ParseLimit.
-      rewrite Slice_App.
-      specialize (Hlim_ok r enc__r Hwf__r Hser__r); rewrite Hlim_ok.
-      rewrite App_nil_l, Drop_App.
-      reflexivity.
-    Qed.
-
-    Lemma SerialLen'Inversion : forall {A : Type} {wfn : nat -> Prop} {wf__a : A -> Prop}
-                                      (ser__n : Serializer nat wfn) (ser__a : Serializer A wf__a)
-                                      (a : A) (enc : Output),
-      SerialLen' ser__n ser__a a = SerialSuccess enc <->
-                                 exists (enc__n enc__a : Output),
-                                   ser__n (Length enc__a) = SerialSuccess enc__n /\
-                                   ser__a a = SerialSuccess enc__a /\
-                                   enc = App enc__n enc__a.
-    Proof using Type.
-      intros. split.
-      - unfold SerialLen'.
-        destruct (ser__a a) as [out__a |] eqn:Ha; last discriminate.
-        destruct (ser__n (Length out__a)) as [out__n |] eqn:Hn; last discriminate.
-        intro H; inversion H as [Henc]; clear H.
-        exists out__n, out__a. repeat (split; done).
-      - intros (out__n & out__a & Hn & Ha & Henc). unfold SerialLen'.
-        rewrite Ha, Hn, Henc. reflexivity.
-    Qed.
+    Definition Len {X : Type} (len : Parser nat) (underlying : Parser X) : Parser X :=
+      Bind len (fun l => Limit underlying l).
 
     (* A parser combinator that makes it possible to transform the result of a parser in another one. *)
-    Definition ParseMap {R U : Type} (underlying : Parser R) (f : R -> U) : Parser U :=
+    Definition Map {A B : Type} (underlying : Parser A) (f : A -> B) : Parser B :=
       fun inp =>
         match underlying inp with
-        | ParseSuccess leftResult remaining => ParseSuccess (f leftResult) remaining
-        | ParseFailure level data => ParseFailure level data
+        | Success result remaining => Success (f result) remaining
+        | Failure level data => Failure level data
         end.
-
-    Definition SerialMap {R U : Type} {wf : U -> Prop} (underlying : Serializer U wf) (f : R -> U) :
-      Serializer R (fun r => wf (f r)) := 
-      fun r => underlying (f r).
 
     (* Returns a parser that succeeds if the underlying parser fails and vice-versa.
      The result does not consume any input. *)
-    Definition Not {R : Type} (underlying : Parser R) : Parser unit :=
+    Definition Not {X : Type} (underlying : Parser X) : Parser unit :=
       fun inp =>
         match underlying inp with
-        | ParseFailure level data as result =>
+        | Failure level data as result =>
             if IsFatalFailure result then
-              PropagateFailure result I
+              Propagate result I
             else
-              ParseSuccess () inp
-        | ParseSuccess _ _ => ParseFailure Recoverable (mkFailureData "not failed" inp None)
+              Success () inp
+        | Success _ _ => Failure Failure.Recoverable (Failure.mkData "Not failed" inp None)
         end.
 
     (* Make the two parsers parse the same string and, if both succeed, return a pair of the
@@ -762,19 +246,19 @@ Module Parsers (InputModule : AbstractInput).
 
      If one parser fails, return that parse failure. If both fail, return the left failure
      *)
-    Definition ParseAnd {L R : Type} (left : Parser L) (right : Parser R) : Parser (L * R) :=
+    Definition And {A B : Type} (left : Parser A) (right : Parser B) : Parser (A * B) :=
       fun inp =>
         match left inp, right inp with
-        | ParseSuccess l _, ParseSuccess r rr => ParseSuccess (l, r) rr
-        | ParseFailure level data, _
-        | _, ParseFailure level data => ParseFailure level data
+        | Success a _, Success b rr => Success (a, b) rr
+        | Failure level data, _
+        | _, Failure level data => Failure level data
         end.
 
-    Definition Or {R : Type} (left : Parser R) (right : Parser R) : Parser R :=
+    Definition Or {X : Type} (left right : Parser X) : Parser X :=
       fun inp =>
         match left inp with
-        | ParseSuccess r rem as p => p
-        | ParseFailure _ data as p =>
+        | Success r rem as p => p
+        | Failure _ data as p =>
             if negb $ NeedsAlternative p inp then
               p
             else 
@@ -782,13 +266,13 @@ Module Parsers (InputModule : AbstractInput).
               if negb $ NeedsAlternative p2 inp then
                 p2
               else
-                MapRecoverableError p2 (fun dataRight => ConcatFailure data dataRight)
+                MapRecoverableError p2 (fun dataRight => Failure.Concat data dataRight)
         end.
 
     (* Like Or, but takes as many parsers as needed *)
-    Fixpoint OrSeq {R : Type} (alternatives : list (Parser R)) : Parser R :=
+    Fixpoint OrSeq {X : Type} (alternatives : list (Parser X)) : Parser X :=
       match alternatives with
-      | [] => ParseFailWith "no alternatives" Recoverable
+      | [] => FailWith "no alternatives" Failure.Recoverable
       | alt :: [] => alt
       | alt :: alts => Or alt (OrSeq alts)
       end.
@@ -797,12 +281,13 @@ Module Parsers (InputModule : AbstractInput).
      If the underlying parser fails,
      - with a fatal failure, return it as-is
      - with a recoverable failure, return it without committing the input *)
-    Definition Lookahead {R : Type} (underlying : Parser R) : Parser R :=
+    Definition Lookahead {X : Type} (underlying : Parser X) : Parser X :=
       fun inp =>
         match underlying inp with
-        | ParseSuccess r rem => ParseSuccess r inp
-        | ParseFailure Fatal data as p => p
-        | ParseFailure Recoverable data => ParseFailure Recoverable (mkFailureData (getFailureMsg data) inp None)
+        | Success r rem => Success r inp
+        | Failure Failure.Fatal data as p => p
+        | Failure Failure.Recoverable data =>
+            Failure Failure.Recoverable (Failure.mkData (Failure.getMsg data) inp None)
         end.
 
     (* (Opt a) evaluates `a` on the input, and then
@@ -811,103 +296,48 @@ Module Parsers (InputModule : AbstractInput).
 
      (Opt a) is useful when there are alternatives to parse and `a` parsed partially and we're OK with
      backtracking to try something else. *)
-    Definition Opt {R : Type} (underlying : Parser R) : Parser R :=
+    Definition Opt {X : Type} (underlying : Parser X) : Parser X :=
       fun inp =>
         match underlying inp with
-        | ParseSuccess r rem as p => p
-        | ParseFailure Fatal data as p => p
-        | ParseFailure Recoverable data => ParseFailure Recoverable (mkFailureData (getFailureMsg data) inp None)
+        | Success r rem as p => p
+        | Failure Failure.Fatal data as p => p
+        | Failure Failure.Recoverable data =>
+            Failure Failure.Recoverable (Failure.mkData (Failure.getMsg data) inp None)
         end.
     
     (* If the condition parser fails, returns a non-committing failure.
      Suitable to use in Or parsers. *)
-    Definition If {L R : Type} (condition : Parser L) (succeed : Parser R) : Parser R :=
-      ParseBind (Lookahead condition) (fun _ => succeed).
+    Definition If {A B : Type} (condition : Parser A) (succeed : Parser B) : Parser B :=
+      Bind (Lookahead condition) (fun _ => succeed).
     
     (* (Maybe a) evaluates `a` on the input, and then
      - If `a` succeeds, wraps the result in Some
      - If `a` fails, and the failure is not fatal and did not consume input, succeeds with None.
        If the error is fatal or did consume input, fails with the same failure. *)
-    Definition Maybe {R : Type} (underlying : Parser R) : Parser (option R) :=
+    Definition Maybe {X : Type} (underlying : Parser X) : Parser (option X) :=
       fun inp =>
         match underlying inp with
-        | ParseSuccess rr rem => ParseSuccess (Some rr) rem
-        | ParseFailure Fatal data as pr => PropagateFailure pr I
-        | ParseFailure Recoverable data as pr => if negb $ NeedsAlternative pr inp then
-                                                  PropagateFailure pr I
-                                                else
-                                                  ParseSuccess None inp
+        | Success rr rem => Success (Some rr) rem
+        | Failure Failure.Fatal data as pr => Propagate pr I
+        | Failure Failure.Recoverable data as pr => if negb $ NeedsAlternative pr inp then
+                                                     Propagate pr I
+                                                   else
+                                                     Success None inp
         end.
 
-    (* TODO debug parser? Might just need to be in OCaml since Rocq I/O functions seem funky *)
-
-    Definition rep'_memory {A : Type} (underlying : Parser A) (inp : Input) : (ParseResult A * bool) :=
+    Program Fixpoint rep' {A B : Type} (underlying : Parser B) (combine : A -> B -> A) (acc : A) (inp : Input)
+      {measure (Length inp)} : Result A :=
       match underlying inp with
-      | ParseSuccess ret rem as p => if Nat.ltb (Length rem) (Length inp) then
-                                      (p, true)
-                                    else
-                                      (p, false)
-      | ParseFailure lvl data as p => (p, true)
+      | Success ret rem => if decide (Length rem < Length inp) then
+                            rep' underlying combine (combine acc ret) rem
+                          else
+                            Success acc inp
+      | Failure lvl data as f => if NeedsAlternative f inp then
+                                  Success acc inp
+                                else
+                                  @Propagate A _ (Failure lvl data) I
       end.
-
-    Lemma rep'_memory_len {A : Type} (underlying : Parser A) (inp : Input) :
-      forall ret rem,
-      rep'_memory underlying inp = (ParseSuccess ret rem, true) -> Length rem < Length inp.
-    Proof using Type.
-      intros ret rem.
-      unfold rep'_memory.
-      destruct (underlying inp) eqn:Hp.
-      - destruct (Length remaining <? Length inp) eqn:Hn.
-        * destruct (Nat.ltb_spec (Length remaining) (Length inp)) in Hn.
-        + intros Hinv. inversion Hinv. subst. assumption.
-        + discriminate.
-          * intros Hinv. inversion Hinv.
-      - intros Hinv. inversion Hinv.
-    Qed.
-
-    (* The primitive repetition combinator which applies the underlying parser over the input
-     until a recoverable failure happens and returns the accumulated results *)
-    (* Defined below, Rep' is the repetition primitive in the parser combinators for Dafny.
-     In this version, we use well-founded recursion to ensure it terminates.
-     In order to the equations plugin to record the decision of the if statement, I'm using
-     decide here, which enables near automatic handling of this fact.
-
-     However, this leads to warnings:
-
-     Warning:
-     The decreasing recursive call obligation Rep'_obligation_2 could not be defined as a hint:
-     Rep'_obligation_2 cannot be used as a hint. [wf-obligation-cannot-be-used,equations,default]
-     Warning:
-     The decreasing recursive call obligation Rep'_obligation_3 could not be defined as a hint:
-     Rep'_obligation_3 cannot be used as a hint. [wf-obligation-cannot-be-used,equations,default]
-
-     I tried to rewrite this to not use `decide`, which resulted in rep'_memory above. The idea
-     there was that since I can use `inspect` and the eqn:H notation to record facts for obligation proofs,
-     the helper function would let me inject the fact that Nat.ltb (Length rem) (Length inp) is true into
-     the obligation context, which I could then solve easily. Unfortunately, this led to the same warnings
-     being issued, so for the moment I've reverted to the self-contained version using decide.
-     *)
-    Equations? rep' {A B : Type} (underlying : Parser B) (combine : A -> B -> A) (acc : A)
-      (inp : Input) : ParseResult A by wf (Length inp) lt :=
-      rep' underlying combine acc inp with underlying inp => {
-        | ParseSuccess ret rem => if decide (Length rem < Length inp) then
-                                   rep' underlying combine (combine acc ret) rem
-                                 else
-                                   ParseSuccess acc inp
-        | ParseFailure lvl data => if NeedsAlternative (ParseFailure lvl data) inp then
-                                    ParseSuccess acc inp
-                                  else
-                                    PropagateFailure (ParseFailure lvl data) I
-        }.
-    Proof.
-      all: try done.
-    Qed.
-
-    (* Proof for the memory version *)
-    (*   apply rep'_memory_len in H. *)
-    (*   assumption. *)
-    (* Qed. *)
-
+                             
     (* Repeats the underlying parser until the first failure that accepts alternatives, combining results
      into an accumulator and return the final accumulated result. *)
     Definition Rep {A B : Type} (underlying : Parser B) (combine : A -> B -> A) (acc : A) :
@@ -918,25 +348,24 @@ Module Parsers (InputModule : AbstractInput).
        final accumulated result. *)
     Fixpoint RepN {A B : Type} (underlying : Parser B) (combine : A -> B -> A) (n : nat) (acc : A) : Parser A :=
       fun inp => match n with
-              | O => ParseSuccess acc inp
+              | O => Success acc inp
               | S m => match underlying inp with
-                      | ParseSuccess b rem => RepN underlying combine m (combine acc b) rem
-                      | ParseFailure lvl data => ParseFailure lvl data
+                      | Success b rem => RepN underlying combine m (combine acc b) rem
+                      | Failure lvl data => Failure lvl data
                       end
               end.
 
     (* Repeats the underlying parser interleaved with a separator. Returns a sequence of results *)
     (* WARN: Unfortunately, without arrays or sequences with constant time accesses accumulating the list
        is an O(n^2) operation *)
-    Definition RepSep {A B : Type} (underlying : Parser A) (separator : Parser B) :
-      Parser (list A) :=
-      ParseBind (Maybe underlying)
+    Definition RepSep {A B : Type} (underlying : Parser A) (separator : Parser B) : Parser (list A) :=
+      Bind (Maybe underlying)
         (fun (result : option A) =>
            match result with
            | Some ret => Rep (ConcatKeepRight separator underlying)
                           (fun (acc : list A) (a : A) => acc ++ [a])
                           [ret]
-           | None => ParseSucceedWith []
+           | None => SucceedWith []
            end).
 
     (* Repeats the underlying parser interleaved with a separator exactly N time.
@@ -944,361 +373,120 @@ Module Parsers (InputModule : AbstractInput).
     (* WARN: Unfortunately, without arrays or sequences with constant time accesses accumulating the list
        is an O(n^2) operation *)
     Definition RepSepN {A B : Type} (underlying : Parser A) (separator : Parser B) (n : nat) : Parser (list A) :=
-      ParseBind (Maybe underlying)
+      Bind (Maybe underlying)
         (fun (result : option A) =>
            match result with
            | Some ret => RepN (ConcatKeepRight separator underlying)
                           (fun (acc : list A) (a : A) => acc ++ [a])
                           (pred n) [ret]
-           | None => ParseSucceedWith []
+           | None => SucceedWith []
         end).
 
     (* Repeats the underlying parser, merging intermediate results. Returns the final merged result. *)
-    Definition RepMerge {A : Type} (underlying : Parser A) (merger : A -> A -> A) : Parser A :=
-      ParseBind (Maybe underlying)
-        (fun (result : option A) =>
+    Definition RepMerge {X : Type} (underlying : Parser X) (merger : X -> X -> X) : Parser X :=
+      Bind (Maybe underlying)
+        (fun (result : option X) =>
            match result with
            | Some ret => Rep underlying merger ret
-           | None => ParseFailWith "No first element in RepMerge" Recoverable
+           | None => FailWith "No first element in RepMerge" Failure.Recoverable
            end).
 
     (* Repeats the underlying parser, merging intermediate results exactly N time.
        Returns the final merged result. *)
-    Definition RepMergeN {A : Type} (underlying : Parser A) (merger : A -> A -> A) (n : nat) : Parser A :=
-      ParseBind (Maybe underlying)
-        (fun (result : option A) =>
+    Definition RepMergeN {X : Type} (underlying : Parser X) (merger : X -> X -> X) (n : nat) : Parser X :=
+      Bind (Maybe underlying)
+        (fun (result : option X) =>
            match result with
            | Some ret => RepN underlying merger (pred n) ret
-           | None => ParseFailWith "No first element in RepMergeN" Recoverable
+           | None => FailWith "No first element in RepMergeN" Failure.Recoverable
            end).
 
     (* Repeats the underlying parser separated by the given separator parser, merging intermediate results.
      Returns the final merged result. *)
-    Definition RepSepMerge {A B : Type} (underlying : Parser A) (separator : Parser B)
-      (merger : A -> A -> A) : Parser A :=
-      ParseBind (Maybe underlying)
+    Definition RepSepMerge {A B : Type} (underlying : Parser A) (separator : Parser B) (merger : A -> A -> A) :
+      Parser A :=
+      Bind (Maybe underlying)
         (fun (result : option A) =>
            match result with
            | Some ret => Rep (ConcatKeepRight separator underlying) merger ret
-           | None => ParseFailWith "No first element in RepSepMerge" Recoverable
+           | None => FailWith "No first element in RepSepMerge" Failure.Recoverable
            end).
 
     (* Repeats the underlying parser separated by the given separator parser, merging intermediate results,
        exactly N times. Returns the final merged result. *)
     Definition RepSepMergeN {A B : Type} (underlying : Parser A) (separator : Parser B)
       (merger : A -> A -> A) (n : nat) : Parser A :=
-      ParseBind (Maybe underlying)
+      Bind (Maybe underlying)
         (fun (result : option A) =>
            match result with
            | Some ret => RepN (ConcatKeepRight separator underlying) merger (pred n) ret
-           | None => ParseFailWith "No first element in RepSepMergeN" Recoverable
+           | None => FailWith "No first element in RepSepMergeN" Failure.Recoverable
            end).
 
     (* Repeated the underlying parser until the first failure that accepts alternatives, and returns the
        underlying sequence. *)
-    Definition ZeroOrMore {R : Type} (underlying : Parser R) : Parser (list R) :=
-      Rep underlying (fun (acc : list R) (r : R) => acc ++ [r]) [].
+    Definition ZeroOrMore {X : Type} (underlying : Parser X) : Parser (list X) :=
+      Rep underlying (fun (acc : list X) (x : X) => acc ++ [x]) [].
 
     (* Like ZeroOrMore but will return a failure if there is not at least one match. *)
-    Definition OneOrMore {R : Type} (underlying : Parser R) : Parser (list R) :=
-      ParseBind underlying
-        (fun r =>
-           Rep underlying (fun (acc : list R) (r : R) => acc ++ [r]) [r]).
+    Definition OneOrMore {X : Type} (underlying : Parser X) : Parser (list X) :=
+      Bind underlying
+        (fun x =>
+           Rep underlying (fun (acc : list X) (x : X) => acc ++ [x]) [x]).
 
-    Definition SeqN {R : Type} (underlying : Parser R) (n : nat) : Parser (list R) :=
-      RepN underlying (fun (acc : list R) (r : R) => acc ++ [r]) n [].
-
-    Fixpoint SerialRepWf {A : Type} (wfa : A -> Prop) (ls : list A) : Prop :=
-      match ls with
-      | [] => True
-      | a :: [] => wfa a
-      | a :: ls => wfa a /\ SerialRepWf wfa ls
-      end.
-
-    Fixpoint sep_rep' {A : Type} {wfa : A -> Prop}
-      (underlying : Serializer A wfa) (acc : Output) : Serializer (list A) (SerialRepWf wfa) :=
-      fun ls =>
-        match ls with
-        | [] => SerialSuccess acc
-        | a :: ls' => match underlying a with
-                     | SerialSuccess a_enc => sep_rep' underlying (App acc a_enc) ls'
-                     | SerialFailure lvl data as f => f
-                     end
-        end.
-
-    Definition SerialRep {A : Type} {wfa : A -> Prop}
-      (underlying : Serializer A wfa) : Serializer (list A) (SerialRepWf wfa) :=
-      fun a => sep_rep' underlying Input_default a.
+    Definition SeqN {X : Type} (underlying : Parser X) (n : nat) : Parser (list X) :=
+      RepN underlying (fun (acc : list X) (x : X) => acc ++ [x]) n [].
 
     Definition RecursiveProgressError {R : Type} (name : string) (inp : Input) (remaining : Input) :
-      ParseResult R :=
+      Result R :=
       if Length remaining == Length inp then
-        ParseFailure Recoverable (mkFailureData (name ++ " no progress in recursive parser") remaining None)
+        Failure Failure.Recoverable (Failure.mkData (name ++ " no progress in recursive parser") remaining None)
       else
-        ParseFailure Fatal (mkFailureData
+        Failure Failure.Fatal (Failure.mkData
                               (name ++ " fixpoint called with an increasing remaining sequence")
                               remaining None).
 
-    Definition par_recur_step {R : Type}
-      (underlying : Parser R -> Parser R)
+    Definition recur_step {X : Type}
+      (underlying : Parser X -> Parser X)
       (inp : Input)
-      (rec_call : forall inp__next : Input, Length inp__next < Length inp -> ParseResult R)
-      (inp__next : Input) : ParseResult R :=
+      (rec_call : forall inp__n : Input, Length inp__n < Length inp -> Result X)
+      (inp__next : Input) : Result X :=
       match decide (Length inp__next < Length inp) with
       | left pf => rec_call inp__next pf
       | right _ => RecursiveProgressError "Parser.Recursive" inp inp__next
       end.
 
-    Program Fixpoint par_recur {R : Type} (underlying : Parser R -> Parser R) (inp : Input)
-      {measure (Length inp)} : ParseResult R :=
-      underlying (par_recur_step underlying inp (fun inp__next _ => par_recur underlying inp__next)) inp.
-    Next Obligation.
-      apply measure_wf.
-      apply lt_wf.
-    Defined.
+    Program Fixpoint recur {X : Type} (underlying : Parser X -> Parser X) (inp : Input)
+      {measure (Length inp)} : Result X :=
+      underlying (recur_step underlying inp (fun inp__n _ => recur underlying inp__n)) inp.
 
     (* Given a function that requires a parser to return a parser, provide the result
        of this parser to that function itself.
 
-       Careful: This function is not tail-recursive.*)
-    Definition ParseRecursive {R : Type} (underlying : Parser R -> Parser R) : Parser R :=
-      par_recur underlying.
+       WARN: This function is not tail-recursive.*)
+    Definition Recursive {X : Type} (underlying : Parser X -> Parser X) : Parser X :=
+      recur underlying.
 
-    Lemma par_recur_unfold {R : Type} (underlying : Parser R -> Parser R) (inp : Input) :
-      par_recur underlying inp =
-      underlying (fun rem => match decide ((Length rem) < (Length inp)) with
-                          | left _ => par_recur underlying rem
-                          | right _ => RecursiveProgressError "Parser.Recursive" inp rem
-                          end) inp.
-    Proof using Type.
-      unfold par_recur at 1. unfold par_recur_func.
-      rewrite WfExtensionality.fix_sub_eq_ext.
-      f_equal.
-    Qed.
-      
-    Definition SerialRecursiveProgressError {R : Type} (name : string) (depth : R -> nat) (r: R) (r__next : R) :
-      SerializeResult :=
-      if depth r__next == depth r then
-        SerialFailure Recoverable (mkFailureData (name ++ " no progress in recursive serializer")
-                                     Input_default None)
-      else
-        SerialFailure Fatal (mkFailureData (name ++ " fixpoint called with deeper value to serialize")
-                               Input_default None).
-
-    Definition ser_recur_step {R : Type} {wfo : R -> Prop}
-      (underlying : Serializer R wfo -> Serializer R wfo)
-      (depth : R -> nat)
-      (r : R)
-      (rec_call : forall r__next : R, depth r__next < depth r -> SerializeResult)
-      (r__next : R) : SerializeResult :=
-      match decide (depth r__next < depth r) with
-      | left pf => rec_call r__next pf
-      | right _ => SerialRecursiveProgressError "Serial.Recursive" depth r r__next
-      end.
-
-    Program Fixpoint ser_recur {R : Type} {wfo : R -> Prop} 
-      (underlying : Serializer R wfo -> Serializer R wfo)
-      (depth : R -> nat) (r : R) {measure (depth r)} : SerializeResult :=
-      underlying (ser_recur_step underlying depth r 
-                    (fun r__next _ => ser_recur underlying depth r__next)) r.
-    Next Obligation.
-      apply measure_wf.
-      apply lt_wf.
-    Defined.
-
-    Definition SerialRecursive {R : Type} {wf : R -> Prop} (underlying : Serializer R wf -> Serializer R wf) depth :
-      Serializer R wf := ser_recur underlying depth.
-
-    Lemma ser_recur_unfold {R : Type} {wfo : R -> Prop} (underlying : Serializer R wfo -> Serializer R wfo)
-      (depth : R -> nat) (r : R) :
-      ser_recur underlying depth r =
-      underlying (fun r__next => match decide (depth r__next < depth r) with
-                            | left _ => ser_recur underlying depth r__next
-                            | right _ => SerialRecursiveProgressError "Serial.Recursive" depth r r__next
-                            end) r.
-    Proof using Type.
-      unfold ser_recur at 1. unfold ser_recur_func.
-      rewrite WfExtensionality.fix_sub_eq_ext.
-      f_equal. 
-    Qed.
-
-    Theorem RecursiveCorrect {R : Type} {wf : R -> Prop}
-      (par_underlying : Parser R -> Parser R)
-      (ser_underlying : Serializer R wf -> Serializer R wf)
-      (depth : R -> nat) :
-      (forall (r : R) (enc rest : Input),
-         wf r ->
-         (forall (inp__next : Input) (r__next : R),
-            Length inp__next < Length (App enc rest) ->
-            depth r__next < depth r ->
-            wf r__next ->
-            forall rest__next,
-            ser_recur ser_underlying depth r__next = SerialSuccess inp__next ->
-            par_recur par_underlying (App inp__next rest__next) = ParseSuccess r__next rest__next) ->
-         ser_underlying (ser_recur_step ser_underlying depth r 
-                           (fun r__next _ => ser_recur ser_underlying depth r__next)) r = SerialSuccess enc ->
-         par_underlying (par_recur_step par_underlying (App enc rest)
-                           (fun inp__next _ => par_recur par_underlying inp__next)) (App enc rest) =
-         ParseSuccess r rest) ->
-      ParseOk (ParseRecursive par_underlying) (SerialRecursive ser_underlying depth).
-    Proof using Type.
-      intros H_underlying_ok.
-      unfold ParseOk, ParseOk', ParseOk'', ParseOk''', ParseRecursive, SerialRecursive.
-      intros x enc rest Hwf Hser.
-      
-      (* The proof proceeds by well-founded induction on depth x *)
-      remember (depth x) as d eqn:Heq.
-      revert x enc rest Hwf Hser Heq.
-      induction d as [d IH] using lt_wf_ind.
-      intros x enc rest Hwf Hser Heq.
-      
-      rewrite par_recur_unfold.
-      rewrite ser_recur_unfold in Hser.
-      
-      unfold par_recur_step in H_underlying_ok.
-      eapply H_underlying_ok; eauto.
-      
-      intros inp__next r__next Hlen Hdepth Hwf__next rest__next Hser__next.
-      
-      eapply IH.
-      - subst d. exact Hdepth.
-      - exact Hwf__next.
-      - exact Hser__next.
-      - reflexivity.
-    Qed.
-
-    Definition par_recur_step_st {R S : Type}
-      (underlying : (S -> Parser R) -> (S -> Parser R))
+    Definition recur_step_st {X S : Type}
+      (underlying : (S -> Parser X) -> (S -> Parser X))
       (inp : Input)
-      (rec_call : forall (st : S) (inp__next : Input), Length inp__next < Length inp ->
-                                                ParseResult R)
+      (rec_call : forall (st : S) (inp__n : Input), Length inp__n < Length inp -> Result X)
       (st : S)
-      (inp__next : Input) : ParseResult R :=
-      match decide (Length inp__next < Length inp) with
-      | left pf => rec_call st inp__next pf
-      | right _ => RecursiveProgressError "Parser.RecursiveState" inp inp__next
+      (inp__n : Input) : Result X :=
+      match decide (Length inp__n < Length inp) with
+      | left pf => rec_call st inp__n pf
+      | right _ => RecursiveProgressError "Parser.RecursiveState" inp inp__n
       end.
 
-    Program Fixpoint par_recur_st {R S : Type}
-      (underlying : (S -> Parser R) -> (S -> Parser R))
-      (st : S) (inp : Input) {measure (Length inp)} : ParseResult R :=
-      underlying (par_recur_step_st underlying inp
-                    (fun st__n inp__next _ => par_recur_st underlying st__n inp__next)) st inp.
-    Next Obligation.
-      apply measure_wf.
-      apply lt_wf.
-    Defined.
+    Program Fixpoint recur_st {X S : Type}
+      (underlying : (S -> Parser X) -> S -> Parser X)
+      (st : S) (inp : Input) {measure (Length inp)} : Result X :=
+      underlying (recur_step_st underlying inp
+                    (fun st__n inp__n _ => recur_st underlying st__n inp__n)) st inp.
 
-    Definition ParseRecursiveState {R S : Type}
-      (underlying : (S -> Parser R) -> (S -> Parser R)) (st : S) : Parser R :=
-      par_recur_st underlying st.
+    Definition RecursiveState {X S : Type}
+      (underlying : (S -> Parser X) -> (S -> Parser X)) (st : S) : Parser X :=
+      recur_st underlying st.
       
-    Lemma par_recur_st_unfold {R S : Type}
-      (underlying : (S -> Parser R) -> (S -> Parser R))
-      (st : S)
-      (inp : Input) :
-      par_recur_st underlying st inp =
-      underlying (fun st__n rem => if decide ((Length rem) < (Length inp)) then
-                                par_recur_st underlying st__n rem
-                              else
-                                RecursiveProgressError "Parser.RecursiveState" inp rem
-        ) st inp.
-    Proof using Type.
-      unfold par_recur_st at 1. unfold par_recur_st_func.
-      rewrite WfExtensionality.fix_sub_eq_ext.
-      f_equal.
-    Qed.
-    
-    Definition ser_recur_step_st {R S : Type} {wfo : R -> Prop}
-      (underlying : (S -> Serializer R wfo) -> S -> Serializer R wfo)
-      (depth : R -> nat)
-      (r : R)
-      (rec_call : forall (st : S) (r__next : R), depth r__next < depth r -> SerializeResult)
-      (st : S)
-      (r__next : R) : SerializeResult :=
-      match decide (depth r__next < depth r) with
-      | left pf => rec_call st r__next pf
-      | right _ => SerialRecursiveProgressError "Serial.RecursiveState" depth r r__next
-      end.
-
-    Program Fixpoint ser_recur_st {R S : Type} {wfo : R -> Prop} 
-      (underlying : (S -> Serializer R wfo) -> S -> Serializer R wfo)
-      (depth : R -> nat) (st : S) (r : R) {measure (depth r)} : SerializeResult :=
-      underlying (ser_recur_step_st underlying depth r 
-                    (fun st__n r__next _ => ser_recur_st underlying depth st__n r__next)) st r.
-    Next Obligation.
-      apply measure_wf.
-      apply lt_wf.
-    Defined.
-
-    Definition SerialRecursiveState {R S : Type} {wf : R -> Prop}
-      (underlying : (S -> Serializer R wf) -> S -> Serializer R wf) depth st :
-      Serializer R wf := ser_recur_st underlying depth st.
-
-    Lemma ser_recur_st_unfold {R S : Type} {wfo : R -> Prop}
-      (underlying : (S -> Serializer R wfo) -> S -> Serializer R wfo)
-      (depth : R -> nat) (st : S) (r : R) :
-      ser_recur_st underlying depth st r =
-      underlying (fun st__n r__next => match decide (depth r__next < depth r) with
-                                | left _ => ser_recur_st underlying depth st__n r__next
-                                | right _ => SerialRecursiveProgressError
-                                              "Serial.RecursiveState" depth r r__next
-                            end) st r.
-    Proof using Type.
-      unfold ser_recur_st at 1. unfold ser_recur_st_func.
-      rewrite WfExtensionality.fix_sub_eq_ext.
-      f_equal. 
-    Qed.
-
-    Theorem RecursiveStateCorrect {R S : Type} {wf : R -> Prop}
-      (par_underlying : (S -> Parser R) -> S -> Parser R)
-      (ser_underlying : (S -> Serializer R wf) -> S -> Serializer R wf)
-      (valid_state : S -> R -> Prop)
-      (depth : R -> nat)
-      (st__init : S)
-      (x : R) :
-      (forall (st : S) (r : R) (enc rest : Input),
-         wf r -> valid_state st r ->
-         (forall (inp__next : Input) (st__next : S) (r__next : R),
-            Length inp__next < Length (App enc rest) ->
-            depth r__next < depth r ->
-            wf r__next ->
-            valid_state st__next r__next ->
-            forall rest__next,
-            ser_recur_st ser_underlying depth st__next r__next = SerialSuccess inp__next ->
-            par_recur_st par_underlying st__next (App inp__next rest__next) = ParseSuccess r__next rest__next) ->
-         ser_underlying (ser_recur_step_st ser_underlying depth r 
-                           (fun st__n r__n _ => ser_recur_st ser_underlying depth st__n r__n)) st r = SerialSuccess enc ->
-         par_underlying (par_recur_step_st par_underlying (App enc rest)
-                           (fun st__n inp__n _ => par_recur_st par_underlying st__n inp__n)) st (App enc rest) =
-         ParseSuccess r rest) ->
-      valid_state st__init x ->
-      ParseOk' (ParseRecursiveState par_underlying st__init)
-        (SerialRecursiveState ser_underlying depth st__init) x.
-    Proof using Type.
-      unfold ParseOk, ParseOk', ParseOk'', ParseOk''', ParseRecursiveState, SerialRecursiveState.
-      intros H_underlying_ok Hstate_valid enc rest Hwf Hser.
-      
-      (* The proof proceeds by well-founded induction on depth x *)
-      remember (depth x) as d eqn:Heq.
-      revert st__init x Hstate_valid enc rest Hwf Hser Heq.
-      induction d as [d IH] using lt_wf_ind.
-      intros st x Hstate enc rest Hwf Hser Heq.
-      
-      rewrite par_recur_st_unfold.
-      rewrite ser_recur_st_unfold in Hser.
-      
-      unfold par_recur_step_st in H_underlying_ok.
-      eapply H_underlying_ok; eauto.
-      
-      intros inp__next st__next r__next Hlen Hdepth Hwf__next Hstate__next rest__next Hser__next.
-      
-      eapply IH.
-      - subst d. exact Hdepth.
-      - exact Hstate__next.
-      - exact Hwf__next.
-      - exact Hser__next.
-      - reflexivity.
-    Qed.
-  End Parsers.
+    End Combinators.
 End Parsers.
