src/parse/Theorems.v
@@ -1,12 +1,468 @@
 From Pollux Require Import Prelude.
 From Pollux.parse Require Import Util.
 From Pollux.parse Require Import Input.
+From Pollux.parse Require Import Failure.
 From Pollux.parse Require Import Parser.
+From Pollux.parse Require Import Serializer.
 
-Module ParseTheorems.
-  Section ParseTheorems.
-    Import Parser.
+From Corelib.Program Require Import Basics Tactics.
+From Stdlib.Program Require Import Program.
 
+Module Theorems (InputModule : AbstractInput).
+  Module F := Failures(InputModule).
+  Module P := Parsers(InputModule).
+  Module S := Serializers(InputModule).
+  Import InputModule.
 
-  End ParseTheorems.
-End ParseTheorems.
+  Definition Output := Input.
+  Definition Parser (X : Type) := P.Parser X.
+  Definition Serializer (X : Type) (wf : X -> Prop) := S.Serializer X wf.
+
+  Definition ParseOk''' {X : Type} {wf : X -> Prop}
+    (par : Parser X) (ser : Serializer X wf) (x : X) (enc rest : Input) :=
+    wf x -> ser x = S.Success enc -> par (App enc rest) = P.Success x rest.
+
+  Definition ParseOk'' {X : Type} {wf : X -> Prop}
+    (par : Parser X) (ser : Serializer X wf) (x : X) (enc : Input) :=
+    forall (rest : Input), ParseOk''' par ser x enc rest.
+
+  Definition ParseOk' {X : Type} {wf : X -> Prop} (par : Parser X) (ser : Serializer X wf) (x : X) :=
+    forall (enc : Input), ParseOk'' par ser x enc.
+
+  Definition ParseOk {X : Type} {wf : X -> Prop} (par : Parser X) (ser : Serializer X wf) :=
+    forall (x : X), ParseOk' par ser x.
+
+  Lemma SucceedCorrect {X : Type} (x : X) :
+    ParseOk' (P.SucceedWith x) S.SucceedWith x.
+  Proof using Type.
+    intros enc rest wf_ok. 
+    unfold S.SucceedWith.
+    intros Hser_ok. inversion Hser_ok as [Henc].
+    unfold P.SucceedWith.
+    rewrite App_nil_l.
+    reflexivity.
+  Qed.
+
+  (* While we couldn't do this for any type (see SucceedCorrect above), we CAN do it with unit
+       since we know statically that there is only one member of type unit, (). *)
+  Lemma EpsilonCorrect : ParseOk P.Epsilon S.Epsilon.
+  Proof using Type.
+    intros x enc rest Hwf Hser_ok.
+    inversion Hser_ok as [Hdefault].
+    subst.
+    unfold P.Epsilon, P.SucceedWith.
+    rewrite App_nil_l.
+    destruct x.
+    reflexivity.
+  Qed.
+
+  Lemma BindCorrect {L R : Type} {wfl : L -> Prop} {wfr : R -> Prop}
+    (lp : Parser L) (ls : R -> S.Serializer L wfl)
+    (rp : L -> Parser R) (rs : S.Serializer R wfr) (tag : R -> L) :
+    forall r, ParseOk lp (ls r) -> ParseOk (rp (tag r)) rs ->
+         ParseOk' (P.Bind lp rp) (S.Bind tag ls rs) r.
+  Proof using Type.
+    intros x Hleft_ok Hright_ok enc rest wf_ok.
+    unfold S.Bind.
+    destruct (ls x (tag x)) as [l_enc|] eqn:Hleft; last discriminate.
+    destruct (rs x) as [r_enc|] eqn:Hright; last discriminate.
+    intro Hser_ok. inversion Hser_ok as [Henc].
+    rewrite App_assoc.
+    unfold P.Bind.
+    destruct wf_ok as [wfl_ok wfr_ok].
+    pose proof Hleft_ok (tag x) l_enc (App r_enc rest) wfl_ok Hleft as Hl_ret.
+    rewrite Hl_ret.
+    pose proof Hright_ok x r_enc rest wfr_ok Hright as Hr_ret.
+    assumption.
+  Qed.
+
+  Definition BindSucceedsRightOk {R L : Type} {wfr : R -> Prop}
+    (rp : L -> Input -> Parser R) (rs : Serializer R wfr) (tag : R -> L) : Prop := 
+    forall (r : R) (r_enc rest : Input), ParseOk''' (rp (tag r) (App r_enc rest)) rs r r_enc rest.
+
+  Definition BindSucceedsLeftOk {R L : Type} {wfl : L -> Prop}
+    (lp : Parser L) (ls : R -> Output -> Serializer L wfl) (tag : R -> L) : Prop :=
+    forall (r : R) (l_enc r_enc rest : Input), ParseOk''' lp (ls r r_enc) (tag r) l_enc (App r_enc rest).
+
+  Lemma BindSucceedsCorrect {L R : Type} {wfl : L -> Prop} {wfr : R -> Prop}
+    (lp : Parser L) (ls : R -> Output -> S.Serializer L wfl)
+    (rp : L -> Input -> Parser R) (rs : S.Serializer R wfr) (tag : R -> L) :
+    BindSucceedsRightOk rp rs tag -> BindSucceedsLeftOk lp ls tag ->
+    ParseOk (P.BindSucceeds lp rp) (S.BindSucceeds tag ls rs).
+  Proof using Type.
+    intros Hright_ok Hleft_ok x enc rest wf_ok.
+    unfold S.BindSucceeds.
+    destruct (rs x) as [r_enc|] eqn:Hright; last discriminate.
+    destruct (ls x r_enc (tag x)) as [l_enc|] eqn:Hleft; last discriminate.
+    intros Hser_ok. inversion Hser_ok as [Henc].
+    destruct wf_ok as [wfl_ok wfr_ok].
+    rewrite App_assoc.
+    unfold P.BindSucceeds.
+    pose proof Hleft_ok x l_enc r_enc rest as Hlp.
+    pose proof wfl_ok as wfl_ok'.
+    apply Hlp in wfl_ok' as _, Hleft as Hl_ret; try assumption.
+    rewrite Hl_ret.
+    pose proof Hright_ok x r_enc rest as Hrp.
+    pose proof wfr_ok as wfr_ok'.
+    apply Hrp in wfr_ok' as _, Hright as Hr_ret; try assumption.
+  Qed.
+
+  Definition BindResultLeftOk {L R : Type} {wfl : L -> Prop} {wfr : R -> Prop}
+    (lp : Parser L) (ls : S.Result -> Output -> Serializer L wfl)
+    (rs : Serializer R wfr) (tag : R -> L): Prop :=
+    forall (r : R), ParseOk' lp (ls (rs r) (S.Out $ rs r)) (tag r).
+
+  Definition BindResultRightOk {L R : Type} {wfr : R -> Prop}
+    (rp : P.Result L -> Input -> Parser R) (rs : Serializer R wfr)
+    (lp : Parser L) (tag : R -> L) : Prop :=
+    forall (r : R) (l_enc r_enc rest: Input),
+    let enc := (App (App l_enc r_enc) rest) in
+    ParseOk''' (rp (lp enc) enc) rs r r_enc rest.
+
+  Lemma BindResultCorrect {L R : Type} {wfl : L -> Prop} {wfr : R -> Prop}
+    (lp : Parser L) (ls : S.Result -> Output -> S.Serializer L wfl)
+    (rp : P.Result L -> Input -> Parser R) (rs : S.Serializer R wfr) (tag : R -> L) :
+    BindResultLeftOk lp ls rs tag -> BindResultRightOk rp rs lp tag ->
+    ParseOk (P.BindResult lp rp) (S.BindResult tag ls rs).
+  Proof using Type.
+    unfold ParseOk, ParseOk', ParseOk'', ParseOk'''.
+    intros Hleft_ok Hright_ok x enc rest wf_ok.
+    unfold S.BindResult.
+    destruct (rs x) as [r_enc|] eqn:Hright.
+    - simpl. symmetry in Hright.
+      intro Hls. unfold S.BindResult_wf in wf_ok.
+      destruct wf_ok as [wfl_ok wfr_ok].
+      pose proof Hright as Hright'.
+      pose proof Hleft_ok x enc rest as Hlp. 
+      rewrite <- Hright in Hlp. simpl in Hlp.
+      pose proof wfl_ok as wfl_ok'.
+      apply Hlp in wfl_ok' as _, Hls as Hl_ret; try assumption.
+      unfold P.BindResult.
+      rewrite Hl_ret.
+
+      unfold BindResultRightOk, ParseOk', ParseOk'', ParseOk''' in Hright_ok.
+      pose proof Hright_ok x enc r_enc rest as Hr.
+      pose proof wfr_ok as wfr_ok'.
+      symmetry in Hright'.
+      apply Hr in wfr_ok' as _, Hright' as Hr_ret; try assumption.
+      (* rewrite Hl_ret in Hr_ret. *)
+  Abort.
+
+  Lemma SerialConcatInversion {A B : Type} {wf__a : A -> Prop} {wf__b : B -> Prop}
+    (ser__a : S.Serializer A wf__a) (ser__b : S.Serializer B wf__b) : 
+    forall (a : A) (b : B) (enc : Output),
+    S.Concat ser__a ser__b (a, b) = S.Success enc <->
+                                  exists (enc__a enc__b : Output),
+                                    ser__a a = S.Success enc__a /\
+                                    ser__b b = S.Success enc__b /\
+                                    enc = App enc__a enc__b.
+  Proof using Type.
+    intros. split.
+    - unfold S.Concat.
+      destruct (ser__a a) as [out__a |] eqn:Ha; last discriminate.
+      destruct (ser__b b) as [out__b |] eqn:Hb; last discriminate.
+      intro H; inversion H as [Henc]; clear H.
+      exists out__a, out__b. repeat (split; first reflexivity); reflexivity.
+    - intros (out__a & out__b & Ha & Hb & Henc). unfold S.Concat.
+      rewrite Ha, Hb. congruence.
+  Qed.
+
+  Theorem ConcatCorrect {L R : Type} {wfl : L -> Prop} {wfr : R -> Prop}
+    (lp : Parser L) (ls : S.Serializer L wfl)
+    (rp : Parser R) (rs : S.Serializer R wfr) :
+    ParseOk lp ls -> ParseOk rp rs -> ParseOk (P.Concat lp rp) (S.Concat ls rs).
+  Proof using Type.
+    intros Hleft_ok Hright_ok.
+    intros [l r] enc rest [Hl_wf Hr_wf] Hconcat.
+    apply SerialConcatInversion in Hconcat.
+    destruct Hconcat as (enc__l & enc__r & Hl & Hr & Henc).
+    subst. rewrite App_assoc.
+    apply (Hleft_ok _ _ (App enc__r rest)) in Hl; last assumption.
+    apply (Hright_ok _ _ rest) in Hr; last assumption.
+    unfold P.Concat.
+    rewrite Hl, Hr.
+    reflexivity.
+  Qed.
+
+  Lemma BindCorrect' {L R : Type} {wfl : L -> Prop} {wfr : R -> Prop}
+    (lp : Parser L) (ls : S.Serializer L wfl)
+    (rp : L -> Parser R) (rs : S.Serializer R wfr) (tag : R -> L) :
+    forall r, ParseOk lp ls -> ParseOk' (rp (tag r)) rs r -> ParseOk' (P.Bind lp rp) (S.Bind' tag ls rs) r.
+  Proof using Type.
+    intros r Hleft_ok Hright_ok enc rest [wfl_ok wfr_ok] Hbind.
+    apply SerialConcatInversion in Hbind.
+    destruct Hbind as (enc__l & enc__r & Hl_ok & Hr_ok & Henc).
+    rewrite Henc. rewrite App_assoc.
+    unfold P.Bind.
+    apply (Hleft_ok _ _ (App enc__r rest)) in Hl_ok; last assumption.
+    rewrite Hl_ok.
+    apply (Hright_ok _ rest) in Hr_ok; assumption.
+  Qed.
+
+  (* Relax the rest requirement, since the Limit parser will ensure rest = [] *)
+  Definition LimitParseOk {X : Type} {wf : X -> Prop} (ser : Serializer X wf) (par : Parser X) := 
+    forall x enc,
+    wf x -> ser x = S.Success enc -> par enc = P.Success x Input_default.
+
+  Definition LenOk {X : Type} {wf : X -> Prop} (ser : Serializer X wf) (len : X -> nat) (x : X) :=
+    forall enc, ser x = S.Success enc -> len x = Length enc.
+
+  Lemma LimitCorrect {X : Type} {wf : X -> Prop} (len : X -> nat)
+    (underlying__ser : S.Serializer X wf) (underlying__par : Parser X) (x : X) :
+    LimitParseOk underlying__ser underlying__par ->
+    LenOk underlying__ser len x ->
+    ParseOk' (P.Limit underlying__par (len x)) (S.Limit underlying__ser len) x.
+  Proof using Type.
+    intros Hlim_ok Hlen_ok enc rest Hwf.
+    unfold S.Limit, P.Limit.
+    intros Hser.
+    unfold LenOk in Hlen_ok.
+    specialize (Hlen_ok enc Hser).
+    rewrite Hlen_ok.
+    rewrite Slice_App.
+    specialize (Hlim_ok x enc Hwf Hser).
+    rewrite Hlim_ok.
+    rewrite Drop_App, App_nil_l.
+    reflexivity.
+  Qed.
+
+  Lemma LenCorrect {X : Type} {wfx : X -> Prop} {wfn : nat -> Prop}
+    (ser__len : S.Serializer nat wfn) (par__len : Parser nat) (len : X -> nat)
+    (ser__x : S.Serializer X wfx) (par__x : Parser X) (x : X) :
+    ParseOk par__len ser__len ->
+    LimitParseOk ser__x par__x ->
+    LenOk ser__x len x ->
+    ParseOk' (P.Len par__len par__x) (S.Len len ser__len ser__x) x.
+  Proof using Type.
+    intros Hnat_ok Hlim_ok Hlen_ok.
+    unfold P.Len, S.Len.
+    apply BindCorrect'; first assumption.
+    apply LimitCorrect; assumption.
+  Qed.
+
+  Definition LimitParseOkWeak {X : Type} {wf : X -> Prop} (ser : Serializer X wf) (par : Parser X) (x : X) := 
+    forall enc, wf x -> ser x = S.Success enc -> par enc = P.Success x Input_default.
+
+  Lemma LenCorrect'Weakened {X : Type} {wfx : X -> Prop} {wfn : nat -> Prop}
+    (ser__len : S.Serializer nat wfn) (par__len : Parser nat)
+    (ser__x : S.Serializer X wfx) (par__x : Parser X) (x : X) :
+    ParseOk par__len ser__len ->
+    LimitParseOkWeak ser__x par__x x ->
+    ParseOk' (P.Len par__len par__x) (S.Len' ser__len ser__x) x.
+  Proof using Type.
+    intros Hnat_ok Hlim_ok enc' rest Hwf.
+    unfold P.Len, S.Len'.
+    destruct (ser__x x) as [enc__x |] eqn:Hser__x; last discriminate.
+    destruct (ser__len (Length enc__x)) as [enc__len |] eqn:Hser__len; last discriminate.
+    unfold S.Len'_wf in Hwf.
+    rewrite Hser__x in Hwf.
+    rewrite Hser__len in Hwf.
+    destruct Hwf as [Hwf__len Hwf__x].
+    intros Henc. inversion Henc as [Henc__x].
+    unfold P.Bind.
+    rewrite App_assoc.
+    specialize (Hnat_ok (Length enc__x) enc__len (App enc__x rest) Hwf__len Hser__len); rewrite Hnat_ok.
+    unfold P.Limit.
+    rewrite Slice_App.
+    specialize (Hlim_ok enc__x Hwf__x Hser__x); rewrite Hlim_ok.
+    rewrite App_nil_l, Drop_App.
+    reflexivity.
+  Qed.
+  
+  Lemma LenCorrect' {X : Type} {wfx : X -> Prop} {wfn : nat -> Prop}
+    (ser__len : S.Serializer nat wfn) (par__len : Parser nat)
+    (ser__x : S.Serializer X wfx) (par__x : Parser X) :
+    ParseOk par__len ser__len ->
+    LimitParseOk ser__x par__x ->
+    ParseOk (P.Len par__len par__x) (S.Len' ser__len ser__x).
+  Proof using Type.
+    intros Hnat_ok Hlim_ok x enc rest Hwf.
+    unfold P.Len, S.Len'.
+    destruct (ser__x x) as [enc__x |] eqn:Hser__x; last discriminate.
+    destruct (ser__len (Length enc__x)) as [enc__len |] eqn:Hser__len; last discriminate.
+    unfold S.Len'_wf in Hwf.
+    rewrite Hser__x in Hwf.
+    rewrite Hser__len in Hwf.
+    destruct Hwf as [Hwf__len Hwf__x].
+    intros H; inversion H as [Henc]; clear H.
+    unfold P.Bind.
+    rewrite App_assoc.
+    specialize (Hnat_ok (Length enc__x) enc__len (App enc__x rest) Hwf__len Hser__len); rewrite Hnat_ok.
+    unfold P.Limit.
+    rewrite Slice_App.
+    specialize (Hlim_ok x enc__x Hwf__x Hser__x); rewrite Hlim_ok.
+    rewrite App_nil_l, Drop_App.
+    reflexivity.
+  Qed.
+
+  Lemma SerialLen'Inversion {X : Type} {wfn : nat -> Prop} {wfx : X -> Prop}
+    (ser__n : S.Serializer nat wfn) (ser__x : S.Serializer X wfx) :
+    forall (x : X) (enc : Output),
+    S.Len' ser__n ser__x x = S.Success enc <->
+                           exists (enc__n enc__x : Output),
+                             ser__n (Length enc__x) = S.Success enc__n /\
+                             ser__x x = S.Success enc__x /\
+                             enc = App enc__n enc__x.
+  Proof using Type.
+    intros. split.
+    - unfold S.Len'.
+      destruct (ser__x x) as [out__x |] eqn:Hx; last discriminate.
+      destruct (ser__n (Length out__x)) as [out__n |] eqn:Hn; last discriminate.
+      intro H; inversion H as [Henc]; clear H.
+      exists out__n, out__x. repeat (split; done).
+    - intros (out__n & out__x & Hn & Hx & Henc). unfold S.Len'.
+      rewrite Hx, Hn, Henc. reflexivity.
+  Qed.
+
+  Lemma par_recur_unfold {X : Type} (underlying : Parser X -> Parser X) (inp : Input) :
+    P.recur underlying inp =
+    underlying (fun rem => match decide (Length rem < Length inp) with
+                        | left _ => P.recur underlying rem
+                        | right _ => P.RecursiveProgressError "Parser.Recursive" inp rem
+                        end) inp.
+  Proof using Type.
+    unfold P.recur at 1. unfold P.recur_func.
+    rewrite WfExtensionality.fix_sub_eq_ext.
+    f_equal.
+  Qed.
+  
+  Lemma ser_recur_unfold {X : Type} {wfx : X -> Prop} (underlying : S.Serializer X wfx -> S.Serializer X wfx)
+    (depth : X -> nat) (x : X) :
+    S.recur underlying depth x =
+    underlying (fun x__n => match decide (depth x__n < depth x) with
+                       | left _ => S.recur underlying depth x__n
+                       | right _ => S.RecursiveProgressError "Serial.Recursive" depth x x__n
+                       end) x.
+  Proof using Type.
+    unfold S.recur at 1. unfold S.recur_func.
+    rewrite WfExtensionality.fix_sub_eq_ext.
+    f_equal. 
+  Qed.
+
+  Theorem RecursiveCorrect {X : Type} {wf : X -> Prop}
+    (par_underlying : Parser X -> Parser X)
+    (ser_underlying : S.Serializer X wf -> S.Serializer X wf)
+    (depth : X -> nat) :
+    (forall (x : X) (enc rest : Input),
+       wf x ->
+       (forall (inp__n : Input) (x__n : X),
+          Length inp__n < Length (App enc rest) ->
+          depth x__n < depth x ->
+          wf x__n ->
+          forall rest__n,
+          S.recur ser_underlying depth x__n = S.Success inp__n ->
+          P.recur par_underlying (App inp__n rest__n) = P.Success x__n rest__n) ->
+       ser_underlying (S.recur_step ser_underlying depth x
+                         (fun x__n _ => S.recur ser_underlying depth x__n)) x = S.Success enc ->
+       par_underlying (P.recur_step par_underlying (App enc rest)
+                         (fun inp__n _ => P.recur par_underlying inp__n)) (App enc rest) =
+       P.Success x rest) ->
+    ParseOk (P.Recursive par_underlying) (S.Recursive ser_underlying depth).
+  Proof using Type.
+    intros H_underlying_ok.
+    unfold ParseOk, ParseOk', ParseOk'', ParseOk''', P.Recursive, S.Recursive.
+    intros x enc rest Hwf Hser.
+    
+    (* The proof proceeds by well-founded induction on depth x *)
+    remember (depth x) as d eqn:Heq.
+    revert x enc rest Hwf Hser Heq.
+    induction d as [d IH] using lt_wf_ind.
+    intros x enc rest Hwf Hser Heq.
+    
+    rewrite par_recur_unfold.
+    rewrite ser_recur_unfold in Hser.
+    
+    unfold P.recur_step in H_underlying_ok.
+    eapply H_underlying_ok; eauto.
+    
+    intros inp__n r__n Hlen__n Hdepth__n Hwf__n rest__n Hser__n.
+    
+    eapply IH.
+    - subst d. exact Hdepth__n.
+    - exact Hwf__n.
+    - exact Hser__n.
+    - reflexivity.
+  Qed.
+
+  Lemma par_recur_st_unfold {X S : Type}
+    (underlying : (S -> Parser X) -> (S -> Parser X))
+    (st : S)
+    (inp : Input) :
+    P.recur_st underlying st inp =
+    underlying (fun st__n rem => if decide (Length rem < Length inp) then
+                              P.recur_st underlying st__n rem
+                            else
+                              P.RecursiveProgressError "Parser.RecursiveState" inp rem
+      ) st inp.
+  Proof using Type.
+    unfold P.recur_st at 1. unfold P.recur_st_func.
+    rewrite WfExtensionality.fix_sub_eq_ext.
+    f_equal.
+  Qed.
+
+  Lemma ser_recur_st_unfold {X S : Type} {wfx : X -> Prop}
+    (underlying : (S -> S.Serializer X wfx) -> S -> S.Serializer X wfx)
+    (depth : X -> nat) (st : S) (x : X) :
+    S.recur_st underlying depth st x =
+    underlying (fun st__n x__n => if decide (depth x__n < depth x) then
+                             S.recur_st underlying depth st__n x__n
+                           else
+                             S.RecursiveProgressError "Serial.RecursiveState" depth x x__n
+      ) st x.
+  Proof using Type.
+    unfold S.recur_st at 1. unfold S.recur_st_func.
+    rewrite WfExtensionality.fix_sub_eq_ext.
+    f_equal. 
+  Qed.
+
+  Theorem RecursiveStateCorrect {X S : Type} {wf : X -> Prop}
+    (par_underlying : (S -> Parser X) -> S -> Parser X)
+    (ser_underlying : (S -> S.Serializer X wf) -> S -> S.Serializer X wf)
+    (valid_state : S -> X -> Prop)
+    (depth : X -> nat)
+    (st : S)
+    (x : X) :
+    (forall (st : S) (x : X) (enc rest : Input),
+       wf x -> valid_state st x ->
+       (forall (inp__n : Input) (st__n : S) (x__n : X),
+          Length inp__n < Length (App enc rest) ->
+          depth x__n < depth x ->
+          wf x__n ->
+          valid_state st__n x__n ->
+          forall rest__n,
+          S.recur_st ser_underlying depth st__n x__n = S.Success inp__n ->
+          P.recur_st par_underlying st__n (App inp__n rest__n) = P.Success x__n rest__n) ->
+       ser_underlying (S.recur_step_st ser_underlying depth x
+                         (fun st__n x__n _ => S.recur_st ser_underlying depth st__n x__n)) st x = S.Success enc ->
+       par_underlying (P.recur_step_st par_underlying (App enc rest)
+                         (fun st__n inp__n _ => P.recur_st par_underlying st__n inp__n)) st (App enc rest) =
+       P.Success x rest) ->
+    valid_state st x ->
+    ParseOk' (P.RecursiveState par_underlying st)
+      (S.RecursiveState ser_underlying depth st) x.
+  Proof using Type.
+    unfold ParseOk, ParseOk', ParseOk'', ParseOk''', P.RecursiveState, S.RecursiveState.
+    intros H_underlying_ok Hstate_valid enc rest Hwf Hser.
+    
+    (* The proof proceeds by well-founded induction on depth x *)
+    remember (depth x) as d eqn:Heq.
+    revert st x Hstate_valid enc rest Hwf Hser Heq.
+    induction d as [d IH] using lt_wf_ind.
+    intros st x Hstate enc rest Hwf Hser Heq.
+    
+    rewrite par_recur_st_unfold.
+    rewrite ser_recur_st_unfold in Hser.
+    
+    unfold P.recur_step_st in H_underlying_ok.
+    eapply H_underlying_ok; eauto.
+    
+    intros inp__n st__n r__n Hlen__n Hdepth__n Hwf__n Hstate__n rest__n Hser__n.
+    
+    eapply IH.
+    - subst d. exact Hdepth__n.
+    - exact Hstate__n.
+    - exact Hwf__n.
+    - exact Hser__n.
+    - reflexivity.
+  Qed.
+End Theorems.
