src/InterParse.v
@@ -1,0 +1,24 @@
+(** Intermediate Parser, building on the Simple Parser and pushing towards Protobuf *)
+
+From Pollux Require Import Prelude.
+From Perennial Require Import Helpers.Word.LittleEndian.
+From Perennial Require Import Helpers.Word.Automation.
+From Stdlib Require Import Structures.Equalities.
+
+From Pollux Require Import Input.
+From Pollux Require Import Failure.
+From Pollux Require Import Parser.
+From Pollux Require Import Serializer.
+From Pollux Require Import Theorems.
+
+Open Scope Z_scope.
+
+Module InterParse.
+  Module F := Failures(ByteInput).
+  Module P := Parsers(ByteInput).
+  Module S := Serializers(ByteInput).
+  Module T := Theorems(ByteInput).
+  Import ByteInput.
+  Import T.
+
+End InterParse.
