src/parse/Failure.v
@@ -1,0 +1,49 @@
+From Pollux Require Import Prelude.
+From Pollux.parse Require Import Util.
+From Pollux.parse Require Import Input.
+
+From Corelib.Program Require Import Basics Tactics.
+From Stdlib.Program Require Import Program.
+
+Module Failures (InputModule : AbstractInput).
+  Section Failure.
+    Import InputModule.
+
+    Context `{EqDecision Input}.
+
+    Inductive Level :=
+    | Fatal
+    | Recoverable.
+
+    (* Record information about when a parse / serialize fails *)
+    (* I'll use the failure data for the serializers too, but interpret "remaining" as "output". *)
+    Inductive Data :=
+    | mkData (msg : string) (remaining : Input) (next : option Data).
+
+    Definition getMsg (data : Data) : string :=
+      match data with
+      | mkData msg _ _ => msg
+      end.
+
+    Definition getRemaining (data : Data) : Input :=
+      match data with
+      | mkData _ remaining _ => remaining
+      end.
+
+    Definition getNext (data : Data) : option Data :=
+      match data with
+      | mkData _ _ next => next
+      end.
+
+    (* Add more failure data to the end of the current chain of failures *)
+    Fixpoint Concat (self other : Data) : Data :=
+      match self with
+      | mkData msg remaining next =>
+          match next with
+          | None => mkData msg remaining (Some other)
+          | Some next_val => mkData msg remaining (Some (Concat next_val other))
+          end
+      end.
+
+  End Failure.
+End Failures.
