src/parse/Serializer.v
@@ -1,0 +1,266 @@
+From Pollux Require Import Prelude.
+From Pollux.parse Require Import Util.
+From Pollux.parse Require Import Input.
+From Pollux.parse Require Import Failure.
+
+From Corelib.Program Require Import Basics Tactics.
+From Stdlib.Program Require Import Program.
+
+Module Serializers (InputModule : AbstractInput).
+  Module Failure := Failures(InputModule).
+  Import InputModule.
+
+  (* Use Output type for serializers *)
+  Definition Output := Input.
+  Definition Output_default := Input_default.
+
+  Section Results.
+    Context `{EqDecision Input}.
+
+    Inductive Result :=
+    | Success (out : Output)
+    | Failure (level : Failure.Level) (data : Failure.Data).
+
+    (** FUNCTIONS ON SERIALIZER RESULTS *)
+
+    Definition Out (sr : Result) : Output := 
+      match sr with
+      | Success out
+      | Failure _ (Failure.mkData _ out _) => out
+      end.
+
+    Definition IsFailure (sr : Result) : bool :=
+      match sr with
+      | Failure _ _ => true
+      | _ => false
+      end.
+    
+    Definition IsFatalFailure (sr : Result) : bool :=
+      match sr with
+      | Failure Failure.Fatal _ => true
+      | _ => false
+      end.
+
+    Definition IsFailureProp (sr : Result) : Prop :=
+      match sr with
+      | Success _ => False
+      | Failure _ _ => True
+      end.
+    
+    Definition IsSuccessProp (sr : Result) : Prop :=
+      match sr with
+      | Success _ => True
+      | Failure _ _ => False
+      end.
+
+  End Results.
+
+  Section Def.
+    Definition Serializer (X : Type) (wf : X -> Prop) := X -> Result. 
+
+    Definition Trivial_wf {X : Type} : X -> Prop := fun _ => True.
+  End Def.
+
+  Section Combinators.
+
+    Definition SucceedWith {X : Type} : Serializer X Trivial_wf :=
+      fun inp => Success Output_default.
+
+    Definition Epsilon : (Serializer unit Trivial_wf) := SucceedWith.
+  
+    Definition FailWith {X : Type} (message : string) (level : Failure.Level) :
+      Serializer X Trivial_wf :=
+        fun inp => Failure level $ Failure.mkData message Output_default None.
+
+    Definition ResultWith {X : Type} (result : Result) : Serializer X Trivial_wf :=
+      fun inp => result.
+
+    Definition Blob : Serializer Output Trivial_wf :=
+      fun b => Success b.
+
+    Definition Concat_wf {L R : Type} (wfl : L -> Prop) (wfr : R -> Prop) : (L * R) -> Prop :=
+      fun lr => let (l, r) := lr in wfl l /\ wfr r.
+
+    Definition Concat {L R : Type} {wfl : L -> Prop} {wfr : R -> Prop}
+      (left : Serializer L wfl) (right : Serializer R wfr) : Serializer (L * R) (Concat_wf wfl wfr) :=
+      fun inp =>
+        let (l, r) := inp in 
+        match left l, right r with
+        | Success l_enc, Success r_enc => Success (App l_enc r_enc)
+        | Failure level data, _
+        | _, Failure level data => Failure level data
+        end.
+
+    Definition Bind'_wf {L R : Type} (wfl : L -> Prop) (wfr : R -> Prop) (tag : R -> L) : R -> Prop :=
+      fun r => wfl (tag r) /\ wfr r.
+
+    Definition Bind' {L R : Type} {wfl : L -> Prop} {wfr : R -> Prop}
+      (tag : R -> L) (left : Serializer L wfl) (right : Serializer R wfr) :
+      Serializer R $ Bind'_wf wfl wfr tag :=
+      fun r => Concat left right (tag r, r).
+
+    Definition Bind_wf {L R : Type} {wfl : L -> Prop} {wfr : R -> Prop}
+      (tag : R -> L) (left : R -> Serializer L wfl) (right : Serializer R wfr) : R -> Prop :=
+      fun r => wfl (tag r) /\ wfr r.
+
+    Definition Bind {L R : Type} {wfl : L -> Prop} {wfr : R -> Prop} 
+      (tag : R -> L) (left : forall r, Serializer L (fun l => l = tag r /\ wfl l)) (right : Serializer R wfr) :
+      Serializer R (@Bind_wf L R wfl wfr tag left right) := 
+      fun r =>
+        match left r (tag r) with
+        | Success l_enc => match right r with
+                          | Success r_enc => Success (App l_enc r_enc)
+                          | Failure lvl data as f => f
+                          end
+        | Failure lvl data as f => f
+        end.
+
+    Definition BindSucceeds_wf {L R : Type} {wfl : L -> Prop} {wfr : R -> Prop}
+      (tag : R -> L) (left : R -> Output -> Serializer L wfl) (right : Serializer R wfr) : R -> Prop :=
+      fun r => wfl (tag r) /\ wfr r.
+
+    (* This is tricky since technically Parse.BindSucceeds isn't limited to only
+    inspecting the encoding of the right serializer (could use things like the
+    lookahead parser) so the correctness theorem will have to ensure that both
+    get the same encoding. *)
+    Definition BindSucceeds {L R : Type} {wfl : L -> Prop} {wfr : R -> Prop}  
+      (tag : R -> L) (left : R -> Output -> Serializer L wfl) (right : Serializer R wfr) :
+      Serializer R (BindSucceeds_wf tag left right) := 
+      fun r =>
+        match right r with
+        | Success r_enc => match left r r_enc (tag r) with
+                          | Success l_enc => Success (App l_enc r_enc)
+                          | Failure lvl data as f => f
+                          end
+        | Failure lvl data as f => f
+        end.
+
+    Definition BindResult_wf {L R : Type} {wfl : L -> Prop} {wfr : R -> Prop}
+      (tag : R -> L) (left : Result -> Output -> Serializer L wfl) (right : Serializer R wfr) :
+      R -> Prop :=
+      fun r => wfl (tag r) /\ wfr r.
+
+    Definition BindResult {L R : Type} {wfl : L -> Prop} {wfr : R -> Prop}
+      (tag : R -> L) (left : Result -> Output -> Serializer L wfl) (right : Serializer R wfr) :
+      Serializer R (BindResult_wf tag left right) :=
+      fun r =>
+        let r_ret := right r in
+        left r_ret (Out r_ret) (tag r).
+
+    (* This formulation is only useful for the proof. *)
+    Definition Limit {X : Type} {wf : X -> Prop} (underlying : Serializer X wf) (len : X -> nat) :
+      Serializer X wf := underlying.
+
+    Definition Len_wf {X : Type} (wfx : X -> Prop) (wfn : nat -> Prop) (len : X -> nat) : X -> Prop :=
+      fun x => wfn (len x) /\ wfx x.
+
+    Definition Len {X : Type} {wfx : X -> Prop} {wfn : nat -> Prop} (len : X -> nat)
+      (ser__len : Serializer nat wfn) (underlying : Serializer X wfx) :
+      Serializer X $ Len_wf wfx wfn len :=
+      Bind' len ser__len $ Limit underlying len.
+
+    Definition Len'_wf {X : Type} {wfx : X -> Prop} {wfn : nat -> Prop}
+      (ser__len : Serializer nat wfn) (ser__x : Serializer X wfx) : X -> Prop :=
+      fun x => match ser__x x with
+            | Success enc__x => match ser__len (Length enc__x) with
+                             | Success enc__len => wfn (Length enc__x) /\ wfx x
+                             | Failure _ _ => True
+                             end
+            | Failure _ _ => True
+            end.
+    
+    Definition Len' {X : Type} {wfx : X -> Prop} {wfn : nat -> Prop}
+      (ser__len : Serializer nat wfn) (underlying : Serializer X wfx) :
+      Serializer X $ Len'_wf ser__len underlying :=
+      fun x => match underlying x with
+            | Success enc => match ser__len (Length enc) with
+                            | Success len_enc => Success (App len_enc enc)
+                            | Failure lvl data as f => f
+                            end
+            | Failure lvl data as f => f
+            end.
+
+    Definition Map_wf {A B : Type} (wf : B -> Prop) (f : A -> B) : A -> Prop :=
+      fun a => wf (f a).
+    
+    Definition Map {A B : Type} {wf : B -> Prop} (underlying : Serializer B wf) (f : A -> B) :
+      Serializer A $ Map_wf wf f := 
+      fun a => underlying (f a).
+
+    Fixpoint Rep_wf {X : Type} (wf : X -> Prop) (ls : list X) : Prop :=
+      match ls with
+      | [] => True
+      | x :: [] => wf x
+      | x :: ls' => wf x /\ Rep_wf wf ls'
+      end.
+
+    Fixpoint rep' {X : Type} {wfx : X -> Prop}
+      (underlying : Serializer X wfx) (acc : Output) : Serializer (list X) (Rep_wf wfx) :=
+      fun ls =>
+        match ls with
+        | [] => Success acc
+        | x :: ls' => match underlying x with
+                     | Success x_enc => rep' underlying (App acc x_enc) ls'
+                     | Failure lvl data as f => f
+                     end
+        end.
+
+    Definition Rep {X : Type} {wfx : X -> Prop}
+      (underlying : Serializer X wfx) : Serializer (list X) (Rep_wf wfx) :=
+      rep' underlying Output_default.
+
+    Definition RecursiveProgressError {X : Type} (name : string) (depth : X -> nat) (x x__n : X) : Result :=
+      if depth x__n == depth x then
+        Failure Failure.Recoverable (Failure.mkData
+                                       (name ++ " no progress in recursive serializer")
+                                       Output_default None)
+      else
+        Failure Failure.Fatal (Failure.mkData
+                                 (name ++ " fixpoint called with deeper value to serialize")
+                                 Output_default None).
+
+    Definition recur_step {X : Type} {wfx : X -> Prop}
+      (underlying : Serializer X wfx -> Serializer X wfx)
+      (depth : X -> nat)
+      (x : X)
+      (rec_call : forall x__n : X, depth x__n < depth x -> Result)
+      (x__n : X) : Result :=
+      match decide (depth x__n < depth x) with
+      | left pf => rec_call x__n pf
+      | right _ => RecursiveProgressError "Serial.Recursive" depth x x__n
+      end.
+
+    Program Fixpoint recur {X : Type} {wfx : X -> Prop} 
+      (underlying : Serializer X wfx -> Serializer X wfx)
+      (depth : X -> nat) (x : X) {measure (depth x)} : Result :=
+      underlying (recur_step underlying depth x
+                    (fun x__n _ => recur underlying depth x__n)) x.
+
+    Definition Recursive {X : Type} {wfx : X -> Prop} (underlying : Serializer X wfx -> Serializer X wfx) depth :
+      Serializer X wfx := recur underlying depth.
+
+    Definition recur_step_st {X S : Type} {wfx : X -> Prop}
+      (underlying : (S -> Serializer X wfx) -> S -> Serializer X wfx)
+      (depth : X -> nat)
+      (x : X)
+      (rec_call : forall (st : S) (x__n : X), depth x__n < depth x -> Result)
+      (st : S)
+      (x__n : X) : Result :=
+      match decide (depth x__n < depth x) with
+      | left pf => rec_call st x__n pf
+      | right _ => RecursiveProgressError "Serial.RecursiveState" depth x x__n
+      end.
+
+    Program Fixpoint recur_st {X S : Type} {wfx : X -> Prop} 
+      (underlying : (S -> Serializer X wfx) -> S -> Serializer X wfx)
+      (depth : X -> nat) (st : S) (x : X) {measure (depth x)} : Result :=
+      underlying (recur_step_st underlying depth x
+                    (fun st__n x__n _ => recur_st underlying depth st__n x__n)) st x.
+
+    Definition RecursiveState {X S : Type} {wfx : X -> Prop}
+      (underlying : (S -> Serializer X wfx) -> S -> Serializer X wfx) depth st :
+      Serializer X wfx := recur_st underlying depth st.
+
+  End Combinators.
+  
+End Serializers.
